Replace Linden characters with Warblre character typeclass

Chars.v
@@ -5,215 +5,203 @@ Import Utils.List.
 From Warblre Require Import Base Typeclasses.
 
 (** * Characters and Strings  *)
-Parameter Char:Type.
-Definition string := list Char.
 
-(* In the semantics, the input string is represented with both the next characters to read
+Section Chars.
+  Context `{characterClass: Character.class}.
+
+  Definition string := list Character.
+
+  (* In the semantics, the input string is represented with both the next characters to read
    and the reversed list of previously read characters (in case we change direction for a lookbehind) *)
-Inductive input : Type :=
-| Input (next: string) (pref: string).
+  Inductive input : Type :=
+  | Input (next: string) (pref: string).
 
-Parameter char_eq_dec : forall (x y : Char), { x = y } + { x <> y }.
-Instance char_EqDec: EqDec Char := EqDec.make Char char_eq_dec.
+  Definition string_eq_dec : forall (x y : string), { x = y } + { x <> y }.
+  Proof.
+    decide equality. apply Character.eq_dec.
+  Defined.
+  #[export] Instance string_EqDec: EqDec string := EqDec.make string string_eq_dec.
 
-Definition string_eq_dec : forall (x y : string), { x = y } + { x <> y }.
-Proof.
-  decide equality. apply char_eq_dec.
-Defined.
-Instance string_EqDec: EqDec string := EqDec.make string string_eq_dec.
-
-Definition input_eq_dec: forall (i1 i2: input), { i1 = i2 } + { i1 <> i2 }.
-Proof. decide equality; apply string_eq_dec. Defined.
-Instance input_EqDec: EqDec input := EqDec.make input input_eq_dec.
+  Definition input_eq_dec: forall (i1 i2: input), { i1 = i2 } + { i1 <> i2 }.
+  Proof. decide equality; apply string_eq_dec. Defined.
+  #[export] Instance input_EqDec: EqDec input := EqDec.make input input_eq_dec.
 
 
-Definition next_str (i:input) : string :=
-  match i with
-  | Input s _ => s
-  end.
+  Definition next_str (i:input) : string :=
+    match i with
+    | Input s _ => s
+    end.
 
-Definition current_str (i:input) (dir: Direction) : string :=
-  match i with
-  | Input next pref =>
-      match dir with forward => next | backward => pref end
-  end.
+  Definition current_str (i:input) (dir: Direction) : string :=
+    match i with
+    | Input next pref =>
+        match dir with forward => next | backward => pref end
+    end.
 
-Definition init_input (str:string) : input :=
-  Input str [].
-
-(** ** Character numeric values *)
-Parameter char_from_numeric_value: nat -> Char.
-Parameter char_numeric_value: Char -> nat.
-Parameter char_numeric_pseudo_bij: forall c, char_from_numeric_value (char_numeric_value c) = c.
-Parameter char_numeric_round_trip_order: forall l r, l <= r -> (char_numeric_value (char_from_numeric_value l)) <= (char_numeric_value (char_from_numeric_value r)).
-
-(** ** Various classes of characters *)
-Parameter char_all: list Char.
-Parameter char_line_terminators: list Char.
-Parameter char_digits: list Char.
-Parameter char_white_spaces: list Char.
-Parameter char_ascii_word_characters: list Char.
-
-(* Deciding whether a character is a word character, to check for word boundaries and for character classes \w and \W *)
-Definition word_char c := inb c char_ascii_word_characters.
-
-(* Axiom specifying that char_all contains all characters *)
-Axiom char_all_in: forall c, In c char_all.
-
-(* Lemma for boolean version of In *)
-Lemma char_all_inb: forall c, inb c char_all = true.
-Proof.
-  intro c. rewrite inb_spec. apply char_all_in.
-Qed.
+  Definition init_input (str:string) : input :=
+    Input str [].
 
 
-(** * Character Descriptors  *)
-(* by character descriptors, we mean everything that can represent a single character *)
-(* the character itself, the dot, an escape, a character group like \d, character classes *)
-Inductive char_descr: Type :=
-| CdEmpty
-| CdDot
-| CdAll
-| CdSingle (c: Char)
-| CdDigits
-| CdWhitespace
-| CdWordChar
-| CdInv (cd: char_descr)
-| CdRange (l h: Char)
-| CdUnion (cd1 cd2: char_descr).
-        
+  (* Deciding whether a character is a word character, to check for word boundaries and for character classes \w and \W *)
+  Definition word_char c := inb c Character.ascii_word_characters.
 
-(*Parameter char_match : Char -> char_descr -> bool.*)
-Fixpoint char_match (c: Char) (cd: char_descr): bool :=
-  match cd with
-  | CdEmpty => false
-  | CdDot => true (* Temporary; at the end, we'd like to take the multiline flag into account *)
-  | CdAll => true
-  | CdSingle c' => c == c'
-  | CdDigits => inb c char_digits
-  | CdWhitespace => inb c char_white_spaces || inb c char_line_terminators
-  | CdWordChar => inb c char_ascii_word_characters (* Temporary; at the end, we'd like to use a rer *)
-  | CdInv cd' => negb (char_match c cd')
-  | CdRange l h => (char_numeric_value l <=? char_numeric_value c) && (char_numeric_value c <=? char_numeric_value h)
-  | CdUnion cd1 cd2 => char_match c cd1 || char_match c cd2
-  end.
+  (* Axiom specifying that char_all contains all characters. TODO Do we want that? *)
+  Axiom char_all_in: forall c, In c Character.all.
+
+  (* Lemma for boolean version of In *)
+  Lemma char_all_inb: forall c, inb c Character.all = true.
+  Proof.
+    intro c. rewrite inb_spec. apply char_all_in.
+  Qed.
 
 
-Lemma single_match:
-  forall c1 c2, char_match c1 (CdSingle c2) = true <-> c1 = c2.
-Proof.
-  intros c1 c2. simpl. apply EqDec.inversion_true.
-Qed.
+  (** * Character Descriptors  *)
+  (* by character descriptors, we mean everything that can represent a single character *)
+  (* the character itself, the dot, an escape, a character group like \d, character classes *)
+  Inductive char_descr: Type :=
+  | CdEmpty
+  | CdDot
+  | CdAll
+  | CdSingle (c: Character)
+  | CdDigits
+  | CdWhitespace
+  | CdWordChar
+  | CdInv (cd: char_descr)
+  | CdRange (l h: Character)
+  | CdUnion (cd1 cd2: char_descr).
 
-Definition char_descr_eq_dec : forall (cd1 cd2: char_descr), { cd1 = cd2 } + { cd1 <> cd2 }.
-Proof. decide equality; apply char_eq_dec. Defined.
+  
+  Fixpoint char_match (c: Character) (cd: char_descr): bool :=
+    match cd with
+    | CdEmpty => false
+    | CdDot => true (* Temporary; at the end, we'd like to take the multiline flag into account *)
+    | CdAll => true
+    | CdSingle c' => c == c'
+    | CdDigits => inb c Character.digits
+    | CdWhitespace => inb c Character.white_spaces || inb c Character.line_terminators
+    | CdWordChar => inb c Character.ascii_word_characters (* Temporary; at the end, we'd like to use a rer *)
+    | CdInv cd' => negb (char_match c cd')
+    | CdRange l h => (Character.numeric_value l <=? Character.numeric_value c) && (Character.numeric_value c <=? Character.numeric_value h)
+    | CdUnion cd1 cd2 => char_match c cd1 || char_match c cd2
+    end.
 
 
-(** * Reading Characters in the String *)
+  Lemma single_match:
+    forall c1 c2, char_match c1 (CdSingle c2) = true <-> c1 = c2.
+  Proof.
+    intros c1 c2. simpl. apply EqDec.inversion_true.
+  Qed.
 
-(* read_char cd i dir returns None if the next character of i with direction dir is accepted by cd *)
-(* otherwise it returns the next input after reading the character, as well as the character actually read *)
-Definition read_char (cd:char_descr) (i:input) (dir: Direction) : option (Char * input) :=
-  match i with
-  | Input next pref =>
-      match dir with
-      | forward =>
-          match next with
-          | [] => None
-          | h::next' => if char_match h cd
-                      then Some (h, Input next' (h::pref))
-                      else None
-          end
-      | backward =>
-          match pref with
-          | [] => None
-          | h::pref' => if char_match h cd
-                      then Some (h, Input (h::next) pref')
-                      else None
-          end
-      end
-  end.
+  Definition char_descr_eq_dec : forall (cd1 cd2: char_descr), { cd1 = cd2 } + { cd1 <> cd2 }.
+  Proof. decide equality; apply Character.eq_dec. Defined.
 
-Inductive ReadResult  : Type :=
-| CanRead
-| CannotRead.
 
-(* the function above is useful when defining trees *)
-(* however, the VMs do it differently: they will test the same character of the input multiple times before advancing *)
-(* instead, we use the two following functions to read and advance *)
+  (** * Reading Characters in the String *)
 
-(* simply checks if the next character of the input corresponds to the given character descriptor *)
-Definition check_read (cd:char_descr) (i:input) (dir: Direction) : ReadResult :=
-  match i with
-  | Input next pref =>
-      match dir with
-      | forward =>
-          match next with
-          | [] => CannotRead
-          | h::next' => if char_match h cd
-                      then CanRead
-                      else CannotRead
-          end
-      | backward =>
-          match pref with
-          | [] => CannotRead
-          | h::pref' => if char_match h cd
-                      then CanRead
-                      else CannotRead
-          end
-      end
-  end.
+  (* read_char cd i dir returns None if the next character of i with direction dir is accepted by cd *)
+  (* otherwise it returns the next input after reading the character, as well as the character actually read *)
+  Definition read_char (cd:char_descr) (i:input) (dir: Direction) : option (Character * input) :=
+    match i with
+    | Input next pref =>
+        match dir with
+        | forward =>
+            match next with
+            | [] => None
+            | h::next' => if char_match h cd
+                        then Some (h, Input next' (h::pref))
+                        else None
+            end
+        | backward =>
+            match pref with
+            | [] => None
+            | h::pref' => if char_match h cd
+                        then Some (h, Input (h::next) pref')
+                        else None
+            end
+        end
+    end.
 
-(* simply advance input to the next character *)
-Definition advance_input (i:input) (dir: Direction) : option input :=
-  match i with
-  | Input next pref =>
-      match dir with
-      | forward =>
-          match next with
-          | [] => None
-          | h::next' => Some (Input next' (h::pref))
-          end
-      | backward =>
-          match pref with
-          | [] => None
-          | h::pref' => Some (Input (h::next) pref')
-          end
-      end
-  end.
+  Inductive ReadResult  : Type :=
+  | CanRead
+  | CannotRead.
 
-(* the proof of equivalence between the two *)
-Theorem can_read_correct:
-  forall i1 cd dir i2,
-  (exists c, read_char cd i1 dir = Some (c, i2)) <->
-    check_read cd i1 dir = CanRead /\ advance_input i1 dir = Some i2.
-Proof.
-  intros i1 cd dir i2. split; intros.
-  - destruct H as [c H].
-    destruct i1. simpl. simpl in H. destruct dir.
-    + destruct next. inversion H. destruct (char_match c0 cd); inversion H; auto.
-    + destruct pref. inversion H. destruct (char_match c0 cd); inversion H; auto.
-  - destruct i1. simpl. simpl in H. destruct dir.
-    + destruct next; inversion H; inversion H1.
-      exists c. destruct (char_match c cd); inversion H0. auto.
-    + destruct pref; inversion H; inversion H1.
-      exists c. destruct (char_match c cd); inversion H0. auto.
-Qed.
+  (* the function above is useful when defining trees *)
+  (* however, the VMs do it differently: they will test the same character of the input multiple times before advancing *)
+  (* instead, we use the two following functions to read and advance *)
 
-Theorem cannot_read_correct:
-  forall i cd dir,
-    read_char cd i dir = None <-> check_read cd i dir = CannotRead.
-Proof.
-  intros i cd dir. destruct i. simpl. destruct dir.
-  - destruct next; split; auto.
-    + destruct (char_match c cd); auto. inversion 1.
-    + destruct (char_match c cd); auto. inversion 1.
-  - destruct pref; split; auto.
-    + destruct (char_match c cd); auto. inversion 1.
-    + destruct (char_match c cd); auto. inversion 1.
-Qed.
+  (* simply checks if the next character of the input corresponds to the given character descriptor *)
+  Definition check_read (cd:char_descr) (i:input) (dir: Direction) : ReadResult :=
+    match i with
+    | Input next pref =>
+        match dir with
+        | forward =>
+            match next with
+            | [] => CannotRead
+            | h::next' => if char_match h cd
+                        then CanRead
+                        else CannotRead
+            end
+        | backward =>
+            match pref with
+            | [] => CannotRead
+            | h::pref' => if char_match h cd
+                        then CanRead
+                        else CannotRead
+            end
+        end
+    end.
 
-(* Inductive relation of next_inputs *)
-Inductive next_input : input -> input -> Direction -> Prop :=
-| nextin: forall i1 i2 dir (ADVANCE: advance_input i1 dir = Some i2),
-    next_input i1 i2 dir.
+  (* Advance input to the next or previous character depending on direction *)
+  Definition advance_input (i:input) (dir: Direction) : option input :=
+    match i with
+    | Input next pref =>
+        match dir with
+        | forward =>
+            match next with
+            | [] => None
+            | h::next' => Some (Input next' (h::pref))
+            end
+        | backward =>
+            match pref with
+            | [] => None
+            | h::pref' => Some (Input (h::next) pref')
+            end
+        end
+    end.
+
+  (* the proof of equivalence between the two *)
+  Theorem can_read_correct:
+    forall i1 cd dir i2,
+    (exists c, read_char cd i1 dir = Some (c, i2)) <->
+      check_read cd i1 dir = CanRead /\ advance_input i1 dir = Some i2.
+  Proof.
+    intros i1 cd dir i2. split; intros.
+    - destruct H as [c H].
+      destruct i1. simpl. simpl in H. destruct dir.
+      + destruct next. inversion H. destruct (char_match t cd); inversion H; auto.
+      + destruct pref. inversion H. destruct (char_match t cd); inversion H; auto.
+    - destruct i1. simpl. simpl in H. destruct dir.
+      + destruct next; inversion H; inversion H1.
+        exists t. destruct (char_match t cd); inversion H0. auto.
+      + destruct pref; inversion H; inversion H1.
+        exists t. destruct (char_match t cd); inversion H0. auto.
+  Qed.
+
+  Theorem cannot_read_correct:
+    forall i cd dir,
+      read_char cd i dir = None <-> check_read cd i dir = CannotRead.
+  Proof.
+    intros i cd dir. destruct i. simpl. destruct dir.
+    - destruct next; split; auto.
+      + destruct (char_match t cd); auto. inversion 1.
+      + destruct (char_match t cd); auto. inversion 1.
+    - destruct pref; split; auto.
+      + destruct (char_match t cd); auto. inversion 1.
+      + destruct (char_match t cd); auto. inversion 1.
+  Qed.
+
+  (* Inductive relation of next_inputs *)
+  Inductive next_input : input -> input -> Direction -> Prop :=
+  | nextin: forall i1 i2 dir (ADVANCE: advance_input i1 dir = Some i2),
+      next_input i1 i2 dir.
+End Chars.
