Regex.v
@@ -38,38 +38,43 @@ Inductive anchor: Type :=
 | WordBoundary
 | NonWordBoundary.
 
-(** * Regex Syntax  *)
-Inductive regex : Type :=
-| Epsilon 
-| Character (cd : char_descr)   (* includes character classes and dot *)
-| Disjunction (r1 r2 : regex) 
-| Sequence (r1 r2 : regex)
-| Quantified (greedy:bool) (min: nat) (plus: non_neg_integer_or_inf) (r1: regex)
-| Lookaround (lk: lookaround) (r: regex)
-| Group (id : group_id) (r : regex)
-| Anchor (a: anchor).
 
-Definition regex_eq_dec : forall (x y : regex), { x = y } + { x <> y }.
-Proof.
-  decide equality.
-  - apply char_descr_eq_dec.
-  - decide equality. apply PeanoNat.Nat.eq_dec.
-  - apply PeanoNat.Nat.eq_dec.
-  - destruct greedy; destruct greedy0; auto. right. lia.
-  - decide equality.
-  - apply PeanoNat.Nat.eq_dec.
-  - decide equality.
-Defined.
+Section Regex.
+  Context `{characterClass: Character.class}.
+  
+  (** * Regex Syntax  *)
+  Inductive regex : Type :=
+  | Epsilon 
+  | Character (cd : char_descr)   (* includes character classes and dot *)
+  | Disjunction (r1 r2 : regex) 
+  | Sequence (r1 r2 : regex)
+  | Quantified (greedy:bool) (min: nat) (plus: non_neg_integer_or_inf) (r1: regex)
+  | Lookaround (lk: lookaround) (r: regex)
+  | Group (id : group_id) (r : regex)
+  | Anchor (a: anchor).
 
-(** * Group Manipulation  *)
+  Definition regex_eq_dec : forall (x y : regex), { x = y } + { x <> y }.
+  Proof.
+    decide equality.
+    - apply char_descr_eq_dec.
+    - decide equality. apply PeanoNat.Nat.eq_dec.
+    - apply PeanoNat.Nat.eq_dec.
+    - destruct greedy; destruct greedy0; auto. right. lia.
+    - decide equality.
+    - apply PeanoNat.Nat.eq_dec.
+    - decide equality.
+  Defined.
 
-(* getting all groups defined in a regex for the reset *)
-Fixpoint def_groups (r:regex) : list group_id :=
-  match r with
-  | Epsilon | Character _  => []
-  | Sequence r1 r2 | Disjunction r1 r2 => def_groups r1 ++ def_groups r2
-  | Quantified _ _ _ r1 => def_groups r1
-  | Lookaround _ r => def_groups r
-  | Group id r1 => id::(def_groups r1)
-  | Anchor _ => []
-  end.
+  (** * Group Manipulation  *)
+
+  (* getting all groups defined in a regex for the reset *)
+  Fixpoint def_groups (r:regex) : list group_id :=
+    match r with
+    | Epsilon | Character _  => []
+    | Sequence r1 r2 | Disjunction r1 r2 => def_groups r1 ++ def_groups r2
+    | Quantified _ _ _ r1 => def_groups r1
+    | Lookaround _ r => def_groups r
+    | Group id r1 => id::(def_groups r1)
+    | Anchor _ => []
+    end.
+End Regex.
