Semantics.v
@@ -10,320 +10,325 @@ From Coq Require Import Lia.
 
 (* This relates a regex and a string to their backtracking tree *)
 
-(** * Lookaround tree correctness  *)
-(* Positive lookarounds expect trees with a result, and negative ones expect trees without results *)
 
-Definition lk_result (lk:lookaround) (t:tree) : Prop :=
-  match (positivity lk) with
-  | true => exists res, first_branch' t = Some res
-  | false => first_branch' t = None
-  end.
+Section Semantics.
+  Context `{characterClass: Character.class}.
+  
+  (** * Lookaround tree correctness  *)
+  (* Positive lookarounds expect trees with a result, and negative ones expect trees without results *)
 
-(** * Anchor semantics *)
+  Definition lk_result (lk:lookaround) (t:tree) : Prop :=
+    match (positivity lk) with
+    | true => exists res, first_branch' t = Some res
+    | false => first_branch' t = None
+    end.
 
-Definition is_boundary (i:input) : bool :=
-  match i with
-  | Input next pref =>
-      match next, pref with
-      | [], [] => false
-      | [], c::p' => word_char c
-      | c::n', [] => word_char c
-      | c1::n', c2::p' =>
-          xorb (word_char c1) (word_char c2)
-      end
-  end.
+  (** * Anchor semantics *)
 
-(* independent of the direction *)
-Definition anchor_satisfied (a:anchor) (i:input) : bool :=
-  match i with
-  | Input next pref =>
-      match a with
-      | BeginInput =>
-          match pref with | [] => true | _ => false end
-      | EndInput =>
-          match next with | [] => true | _ => false end
-      | WordBoundary =>
-          is_boundary i
-      | NonWordBoundary =>
-          negb (is_boundary i)
-      end
-  end.
+  Definition is_boundary (i:input) : bool :=
+    match i with
+    | Input next pref =>
+        match next, pref with
+        | [], [] => false
+        | [], c::p' => word_char c
+        | c::n', [] => word_char c
+        | c1::n', c2::p' =>
+            xorb (word_char c1) (word_char c2)
+        end
+    end.
 
-
-(** * Continuation Semantics *)
-
-(* actions are things to do after executing the current focused regex *)
-(* it can either be executing another regex (encoding the sequence) *)
-(* or checking that the current string is different from another string (for the JS star) *)
-(* or closing a group after it's been opened *)
-Inductive action: Type :=
-| Areg: regex -> action
-| Acheck: string -> action
-| Aclose: group_id -> action.
-
-Definition continuation: Type := list action.
-
-(* `is_tree r cont str t` means that `t` is a correct backtracking tree for `r` on `s`,
-   where we have to execute `cont` at each leaf *)
-Inductive is_tree: regex -> continuation -> input -> Direction -> tree -> Prop :=
-| tree_epsilon:
-  (* on an empty continuation *)
-  forall inp dir,
-    is_tree Epsilon [] inp dir Match
-| tree_pop_reg:
-  (* pops a regex from the continuation list *)
-  forall inp dir regcont tailcont treecont
-    (TREECONT: is_tree regcont tailcont inp dir treecont),
-    is_tree Epsilon (Areg regcont :: tailcont) inp dir treecont
-| tree_pop_check:
-(* pops a successful check from the continuation list *)
-  forall inp dir strcheck tailcont treecont
-    (PROGRESS: current_str inp dir <> strcheck)
-    (TREECONT: is_tree Epsilon tailcont inp dir treecont),
-    is_tree Epsilon (Acheck strcheck :: tailcont) inp dir (CheckPass strcheck treecont)
-| tree_pop_check_fail:
-(* pops a failing check from the continuation list *)
-  forall inp dir strcheck tailcont
-    (CHECKFAIL: current_str inp dir = strcheck),
-    is_tree Epsilon (Acheck strcheck :: tailcont) inp dir (CheckFail strcheck)
-| tree_pop_close:
-(* pops the closing of a group from the continuation list *)
-  forall inp dir tailcont treecont gid
-    (TREECONT: is_tree Epsilon tailcont inp dir treecont),
-    is_tree Epsilon (Aclose gid :: tailcont) inp dir (GroupAction (Close gid) treecont)
-| tree_char:
-  forall c cd inp nextinp dir cont tcont
-    (READ: read_char cd inp dir = Some (c, nextinp))
-    (TREECONT: is_tree Epsilon cont nextinp dir tcont),
-    is_tree (Regex.Character cd) cont inp dir (Read c tcont)
-| tree_char_fail:
-  forall cd inp dir cont
-    (READ: read_char cd inp dir = None),
-    is_tree (Regex.Character cd) cont inp dir Mismatch
-| tree_disj:
-  forall r1 r2 cont t1 t2 inp dir
-    (ISTREE1: is_tree r1 cont inp dir t1)
-    (ISTREE2: is_tree r2 cont inp dir t2),
-    is_tree (Disjunction r1 r2) cont inp dir (Choice t1 t2)
-| tree_sequence_fwd:
-  (* adding next regex to the continuation *)
-  forall r1 r2 cont t inp
-    (CONT: is_tree r1 (Areg r2 :: cont) inp forward t),
-    is_tree (Sequence r1 r2) cont inp forward t
-| tree_sequence_bwd:
-  (* adding next regex to the continuation, reversing the order of regexes *)
-  forall r1 r2 cont t inp
-    (CONT: is_tree r2 (Areg r1 :: cont) inp backward t),
-    is_tree (Sequence r1 r2) cont inp backward t
-| tree_quant_minpos:
-  forall r1 greedy min plus cont titer inp dir gidl
-    (* the list of capture groups to reset *)
-    (RESET: gidl = def_groups r1)
-    (* doing one iteration *)
-    (ISTREE1: is_tree r1 (Areg (Quantified greedy min plus r1)::cont) inp dir titer),
-    is_tree (Quantified greedy (S min) plus r1) cont inp dir (GroupAction (Reset gidl) titer)
-| tree_quant_minzero_pluszero:
-  forall r1 greedy cont tskip inp dir
-    (SKIP: is_tree Epsilon cont inp dir tskip),
-    is_tree (Quantified greedy 0 (NoI.N 0) r1) cont inp dir tskip
-| tree_quant_minzero_pluspos:
-  forall r1 greedy plus cont titer tskip tquant inp dir gidl
-    (* the list of capture groups to reset *)
-    (RESET: gidl = def_groups r1)
-    (* doing one iteration, then a check, then executing the next quantifier *)
-    (ISTREE1: is_tree r1 (Acheck (current_str inp dir)::Areg (Quantified greedy 0 plus r1)::cont) inp dir titer)
-    (* skipping the quantifier entirely *)
-    (SKIP: is_tree Epsilon cont inp dir tskip)
-    (CHOICE: tquant = greedy_choice greedy (GroupAction (Reset gidl) titer) tskip),
-    is_tree (Quantified greedy 0 (NoI.N 1 + plus)%NoI r1) cont inp dir tquant
-| tree_group:
-  forall r1 cont treecont inp dir gid
-    (TREECONT: is_tree r1 (Aclose gid :: cont) inp dir treecont),
-    is_tree (Group gid r1) cont inp dir (GroupAction (Open gid) treecont)
-| tree_lk:
-  forall lk r1 cont treecont treelk inp dir
-    (* there is a tree for the lookaround *)
-    (TREELK: is_tree r1 [] inp (lk_dir lk) treelk)
-  (* this tree has the correct expected result (positivity) *)
-    (RES_LK: lk_result lk treelk)
-    (TREECONT: is_tree Epsilon cont inp dir treecont),
-    is_tree (Lookaround lk r1) cont inp dir (LK lk treelk treecont)
-| tree_lk_fail:
-  forall lk r1 cont treelk inp dir
-    (TREELK: is_tree r1 [] inp (lk_dir lk) treelk)
-    (FAIL_LK: ~ lk_result lk treelk),
-    is_tree (Lookaround lk r1) cont inp dir (LKFail lk treelk)
-| tree_anchor:
-  forall a cont treecont inp dir
-    (ANCHOR: anchor_satisfied a inp = true)
-    (TREECONT: is_tree Epsilon cont inp dir treecont),
-    is_tree (Anchor a) cont inp dir (AnchorPass a treecont)
-| tree_anchor_fail:
-  forall a cont inp dir
-    (ANCHOR: anchor_satisfied a inp = false),
-    is_tree (Anchor a) cont inp dir (AnchorFail a).
+  (* independent of the direction *)
+  Definition anchor_satisfied (a:anchor) (i:input) : bool :=
+    match i with
+    | Input next pref =>
+        match a with
+        | BeginInput =>
+            match pref with | [] => true | _ => false end
+        | EndInput =>
+            match next with | [] => true | _ => false end
+        | WordBoundary =>
+            is_boundary i
+        | NonWordBoundary =>
+            negb (is_boundary i)
+        end
+    end.
 
 
-Definition backtree (r:regex) (str:string) (t:tree): Prop :=
-  is_tree r [] (init_input str) forward t.
+  (** * Continuation Semantics *)
 
-(* Adding Epsilon to the list of continuations *)
-(*Lemma is_tree_eps':
-  forall reg cont inp t, is_tree reg cont inp t -> forall cont1 cont2, cont = cont1 ++ (Areg Epsilon::cont2) -> is_tree reg (cont1 ++ cont2) inp t.
-Proof.
-  intros reg cont inp t His_tree.
-  induction His_tree.
-  (* TODO From now *)
-  - (* tree_epsilon *)
-    intros cont1 cont2 Habs. destruct cont1; discriminate.
-  - (* tree_pop_reg *)
-    intros cont1 cont2 H. destruct cont1 as [|x cont1].
-    + inversion H. subst. assumption.
-    + simpl in *. inversion H. subst. apply tree_pop_reg. apply IHHis_tree. reflexivity.
-  - (* tree_pop_check *)
-    intros cont1 cont2 H. destruct cont1 as [|x cont1].
-    + inversion H.
-    + simpl in H. inversion H. simpl. apply tree_pop_check.
-      * assumption.
-      * apply IHHis_tree. assumption.
-  - (* tree_pop_check_fail *)
-    intros [|x cont1] cont2 H; simpl in *.
-    + inversion H.
-    + inversion H. apply tree_pop_check_fail. assumption.
-  - (* tree_pop_close *)
-    intros [|x cont1] cont2 H; simpl in *.
-    + inversion H.
-    + inversion H. apply tree_pop_close. apply IHHis_tree. assumption.
-  - (* tree_char *)
-    intros cont1 cont2 H.
-    eapply tree_char.
-    + apply READ.
-    + apply IHHis_tree. apply H.
-  - (* tree_char_fail *)
-    intros cont1 cont2 H. apply tree_char_fail. apply READ.
-  - (* tree_disj *)
-    intros cont1 cont2 H.
-    apply tree_disj.
-    + apply IHHis_tree1. apply H.
-    + apply IHHis_tree2. apply H.
-  - (* tree_sequence *)
-    intros cont1 cont2 H.
-    apply tree_sequence.
-    subst cont.
-    rewrite app_comm_cons.
-    apply IHHis_tree.
-    simpl. reflexivity.
-  - (* tree_star *)
-    intros cont1 cont2 H.
-    eapply tree_star.
-    + apply RESET.
-    + subst cont.
-      rewrite app_comm_cons. rewrite app_comm_cons.
-      rewrite app_comm_cons in IHHis_tree1. rewrite app_comm_cons in IHHis_tree1.
-      apply IHHis_tree1. reflexivity.
-    + apply IHHis_tree2. assumption.
-    + assumption.
-  - (* tree_group *)
-    intros cont1 cont2 H.
-    subst cont.
-    apply tree_group.
-    rewrite app_comm_cons.
-    apply IHHis_tree.
-    simpl. reflexivity.
-Qed.
+  (* actions are things to do after executing the current focused regex *)
+  (* it can either be executing another regex (encoding the sequence) *)
+  (* or checking that the current string is different from another string (for the JS star) *)
+  (* or closing a group after it's been opened *)
+  Inductive action: Type :=
+  | Areg: regex -> action
+  | Acheck: string -> action
+  | Aclose: group_id -> action.
 
-Corollary is_tree_eps:
-  forall reg cont1 cont2 inp t, is_tree reg (cont1 ++ Areg Epsilon :: cont2) inp t -> is_tree reg (cont1 ++ cont2) inp t.
-Proof.
-  intros reg cont1 cont2 inp t H.
-  eapply is_tree_eps'.
-  - apply H.
-  - reflexivity.
-Qed.*)
+  Definition continuation: Type := list action.
 
-
-(** * Determinism  *)
-
-Theorem is_tree_determ:
-  forall r cont i dir t1 t2,
-    is_tree r cont i dir t1 ->
-    is_tree r cont i dir t2 ->
-    t1 = t2.
-Proof.
-  intros r cont i dir t1 t2 H.
-  generalize dependent t2.
-  induction H; intros.
-  - inversion H; subst; auto.
-  - inversion H0; subst; auto.
-  - inversion H0; subst; auto.
-    + apply IHis_tree in TREECONT. subst. auto.
-    + exfalso. apply PROGRESS. auto.
-  - inversion H; subst; auto.
-    exfalso. apply PROGRESS. auto.
-  - inversion H0; subst; auto.
-    apply IHis_tree in TREECONT. subst. auto.
-  - inversion H0; subst; auto; rewrite READ0 in READ; inversion READ; subst.
-    apply IHis_tree in TREECONT. subst. auto.
-  - inversion H; subst; auto.
-    rewrite READ0 in READ. inversion READ.
-  - inversion H1; subst; auto.
-    apply IHis_tree1 in ISTREE1. apply IHis_tree2 in ISTREE2. subst. auto.
-  - inversion H0; subst; auto.
-  - inversion H0; subst; auto.
-  - inversion H0; subst; auto.
-    apply IHis_tree in ISTREE1.
-    subst. auto.
-  - inversion H0; subst; auto.
-    destruct plus; discriminate.
-  - inversion H1; subst; auto.
-    + destruct plus; discriminate.
-    + apply plus_one_inj in H4. subst plus0.
-      apply IHis_tree1 in ISTREE1. apply IHis_tree2 in SKIP. subst. auto.
-  - inversion H0; subst; auto.
-    apply IHis_tree in TREECONT. subst. auto.
-  (* Following two bullets copied from backtree repo *)
-  - inversion H1; subst; auto.
-    2: { apply IHis_tree1 in TREELK. subst. exfalso. apply FAIL_LK. auto. }
-    apply IHis_tree1 in TREELK. apply IHis_tree2 in TREECONT. subst. auto.
-  - inversion H0; subst; auto.
-    { apply IHis_tree in TREELK. subst. exfalso. apply FAIL_LK. auto. }
-    apply IHis_tree in TREELK. subst. auto.
-  - inversion H0; subst; auto.
-    + f_equal. auto.
-    + congruence.
-  - inversion H; subst; auto. congruence.
-Qed.
-
-Corollary backtree_determ:
-  forall r s t1 t2,
-    backtree r s t1 ->
-    backtree r s t2 ->
-    t1 = t2.
-Proof.
-  unfold backtree. intros r s t1 t2 H H0. eapply is_tree_determ; eauto.
-Qed.
-
-(* We could also prove that there always exists a backtree for any regexes and string,
- bu that amounts to proving the termination of the backtree construction. *)
+  (* `is_tree r cont str t` means that `t` is a correct backtracking tree for `r` on `s`,
+     where we have to execute `cont` at each leaf *)
+  Inductive is_tree: regex -> continuation -> input -> Direction -> tree -> Prop :=
+  | tree_epsilon:
+    (* on an empty continuation *)
+    forall inp dir,
+      is_tree Epsilon [] inp dir Match
+  | tree_pop_reg:
+    (* pops a regex from the continuation list *)
+    forall inp dir regcont tailcont treecont
+      (TREECONT: is_tree regcont tailcont inp dir treecont),
+      is_tree Epsilon (Areg regcont :: tailcont) inp dir treecont
+  | tree_pop_check:
+  (* pops a successful check from the continuation list *)
+    forall inp dir strcheck tailcont treecont
+      (PROGRESS: current_str inp dir <> strcheck)
+      (TREECONT: is_tree Epsilon tailcont inp dir treecont),
+      is_tree Epsilon (Acheck strcheck :: tailcont) inp dir (CheckPass strcheck treecont)
+  | tree_pop_check_fail:
+  (* pops a failing check from the continuation list *)
+    forall inp dir strcheck tailcont
+      (CHECKFAIL: current_str inp dir = strcheck),
+      is_tree Epsilon (Acheck strcheck :: tailcont) inp dir (CheckFail strcheck)
+  | tree_pop_close:
+  (* pops the closing of a group from the continuation list *)
+    forall inp dir tailcont treecont gid
+      (TREECONT: is_tree Epsilon tailcont inp dir treecont),
+      is_tree Epsilon (Aclose gid :: tailcont) inp dir (GroupAction (Close gid) treecont)
+  | tree_char:
+    forall c cd inp nextinp dir cont tcont
+      (READ: read_char cd inp dir = Some (c, nextinp))
+      (TREECONT: is_tree Epsilon cont nextinp dir tcont),
+      is_tree (Regex.Character cd) cont inp dir (Read c tcont)
+  | tree_char_fail:
+    forall cd inp dir cont
+      (READ: read_char cd inp dir = None),
+      is_tree (Regex.Character cd) cont inp dir Mismatch
+  | tree_disj:
+    forall r1 r2 cont t1 t2 inp dir
+      (ISTREE1: is_tree r1 cont inp dir t1)
+      (ISTREE2: is_tree r2 cont inp dir t2),
+      is_tree (Disjunction r1 r2) cont inp dir (Choice t1 t2)
+  | tree_sequence_fwd:
+    (* adding next regex to the continuation *)
+    forall r1 r2 cont t inp
+      (CONT: is_tree r1 (Areg r2 :: cont) inp forward t),
+      is_tree (Sequence r1 r2) cont inp forward t
+  | tree_sequence_bwd:
+    (* adding next regex to the continuation, reversing the order of regexes *)
+    forall r1 r2 cont t inp
+      (CONT: is_tree r2 (Areg r1 :: cont) inp backward t),
+      is_tree (Sequence r1 r2) cont inp backward t
+  | tree_quant_minpos:
+    forall r1 greedy min plus cont titer inp dir gidl
+      (* the list of capture groups to reset *)
+      (RESET: gidl = def_groups r1)
+      (* doing one iteration *)
+      (ISTREE1: is_tree r1 (Areg (Quantified greedy min plus r1)::cont) inp dir titer),
+      is_tree (Quantified greedy (S min) plus r1) cont inp dir (GroupAction (Reset gidl) titer)
+  | tree_quant_minzero_pluszero:
+    forall r1 greedy cont tskip inp dir
+      (SKIP: is_tree Epsilon cont inp dir tskip),
+      is_tree (Quantified greedy 0 (NoI.N 0) r1) cont inp dir tskip
+  | tree_quant_minzero_pluspos:
+    forall r1 greedy plus cont titer tskip tquant inp dir gidl
+      (* the list of capture groups to reset *)
+      (RESET: gidl = def_groups r1)
+      (* doing one iteration, then a check, then executing the next quantifier *)
+      (ISTREE1: is_tree r1 (Acheck (current_str inp dir)::Areg (Quantified greedy 0 plus r1)::cont) inp dir titer)
+      (* skipping the quantifier entirely *)
+      (SKIP: is_tree Epsilon cont inp dir tskip)
+      (CHOICE: tquant = greedy_choice greedy (GroupAction (Reset gidl) titer) tskip),
+      is_tree (Quantified greedy 0 (NoI.N 1 + plus)%NoI r1) cont inp dir tquant
+  | tree_group:
+    forall r1 cont treecont inp dir gid
+      (TREECONT: is_tree r1 (Aclose gid :: cont) inp dir treecont),
+      is_tree (Group gid r1) cont inp dir (GroupAction (Open gid) treecont)
+  | tree_lk:
+    forall lk r1 cont treecont treelk inp dir
+      (* there is a tree for the lookaround *)
+      (TREELK: is_tree r1 [] inp (lk_dir lk) treelk)
+    (* this tree has the correct expected result (positivity) *)
+      (RES_LK: lk_result lk treelk)
+      (TREECONT: is_tree Epsilon cont inp dir treecont),
+      is_tree (Lookaround lk r1) cont inp dir (LK lk treelk treecont)
+  | tree_lk_fail:
+    forall lk r1 cont treelk inp dir
+      (TREELK: is_tree r1 [] inp (lk_dir lk) treelk)
+      (FAIL_LK: ~ lk_result lk treelk),
+      is_tree (Lookaround lk r1) cont inp dir (LKFail lk treelk)
+  | tree_anchor:
+    forall a cont treecont inp dir
+      (ANCHOR: anchor_satisfied a inp = true)
+      (TREECONT: is_tree Epsilon cont inp dir treecont),
+      is_tree (Anchor a) cont inp dir (AnchorPass a treecont)
+  | tree_anchor_fail:
+    forall a cont inp dir
+      (ANCHOR: anchor_satisfied a inp = false),
+      is_tree (Anchor a) cont inp dir (AnchorFail a).
 
 
-(** * Backtracking  *)
-(* the result of backtracking is just the first branch of the corresponding tree *)
+  Definition backtree (r:regex) (str:string) (t:tree): Prop :=
+    is_tree r [] (init_input str) forward t.
 
-Inductive backtracking_result: regex -> string -> option leaf -> Prop :=
-| bt_result:
-  forall r str res tree
-    (TREE: backtree r str tree)
-    (FIRST: first_branch tree = res),
-    backtracking_result r str res.
+  (* Adding Epsilon to the list of continuations *)
+  (*Lemma is_tree_eps':
+    forall reg cont inp t, is_tree reg cont inp t -> forall cont1 cont2, cont = cont1 ++ (Areg Epsilon::cont2) -> is_tree reg (cont1 ++ cont2) inp t.
+  Proof.
+    intros reg cont inp t His_tree.
+    induction His_tree.
+    (* TODO From now *)
+    - (* tree_epsilon *)
+      intros cont1 cont2 Habs. destruct cont1; discriminate.
+    - (* tree_pop_reg *)
+      intros cont1 cont2 H. destruct cont1 as [|x cont1].
+      + inversion H. subst. assumption.
+      + simpl in *. inversion H. subst. apply tree_pop_reg. apply IHHis_tree. reflexivity.
+    - (* tree_pop_check *)
+      intros cont1 cont2 H. destruct cont1 as [|x cont1].
+      + inversion H.
+      + simpl in H. inversion H. simpl. apply tree_pop_check.
+        * assumption.
+        * apply IHHis_tree. assumption.
+    - (* tree_pop_check_fail *)
+      intros [|x cont1] cont2 H; simpl in *.
+      + inversion H.
+      + inversion H. apply tree_pop_check_fail. assumption.
+    - (* tree_pop_close *)
+      intros [|x cont1] cont2 H; simpl in *.
+      + inversion H.
+      + inversion H. apply tree_pop_close. apply IHHis_tree. assumption.
+    - (* tree_char *)
+      intros cont1 cont2 H.
+      eapply tree_char.
+      + apply READ.
+      + apply IHHis_tree. apply H.
+    - (* tree_char_fail *)
+      intros cont1 cont2 H. apply tree_char_fail. apply READ.
+    - (* tree_disj *)
+      intros cont1 cont2 H.
+      apply tree_disj.
+      + apply IHHis_tree1. apply H.
+      + apply IHHis_tree2. apply H.
+    - (* tree_sequence *)
+      intros cont1 cont2 H.
+      apply tree_sequence.
+      subst cont.
+      rewrite app_comm_cons.
+      apply IHHis_tree.
+      simpl. reflexivity.
+    - (* tree_star *)
+      intros cont1 cont2 H.
+      eapply tree_star.
+      + apply RESET.
+      + subst cont.
+        rewrite app_comm_cons. rewrite app_comm_cons.
+        rewrite app_comm_cons in IHHis_tree1. rewrite app_comm_cons in IHHis_tree1.
+        apply IHHis_tree1. reflexivity.
+      + apply IHHis_tree2. assumption.
+      + assumption.
+    - (* tree_group *)
+      intros cont1 cont2 H.
+      subst cont.
+      apply tree_group.
+      rewrite app_comm_cons.
+      apply IHHis_tree.
+      simpl. reflexivity.
+  Qed.
 
-Lemma backtracking_determ:
-  forall r str res1 res2,
-    backtracking_result r str res1 ->
-    backtracking_result r str res2 ->
-    res1 = res2.
-Proof.
-  intros r str res1 res2 H H0. inversion H. subst.
-  inversion H0. subst.
-  specialize (backtree_determ _ _ _ _ TREE TREE0). intros. subst. auto.
-Qed.
+  Corollary is_tree_eps:
+    forall reg cont1 cont2 inp t, is_tree reg (cont1 ++ Areg Epsilon :: cont2) inp t -> is_tree reg (cont1 ++ cont2) inp t.
+  Proof.
+    intros reg cont1 cont2 inp t H.
+    eapply is_tree_eps'.
+    - apply H.
+    - reflexivity.
+  Qed.*)
+
+
+  (** * Determinism  *)
+
+  Theorem is_tree_determ:
+    forall r cont i dir t1 t2,
+      is_tree r cont i dir t1 ->
+      is_tree r cont i dir t2 ->
+      t1 = t2.
+  Proof.
+    intros r cont i dir t1 t2 H.
+    generalize dependent t2.
+    induction H; intros.
+    - inversion H; subst; auto.
+    - inversion H0; subst; auto.
+    - inversion H0; subst; auto.
+      + apply IHis_tree in TREECONT. subst. auto.
+      + exfalso. apply PROGRESS. auto.
+    - inversion H; subst; auto.
+      exfalso. apply PROGRESS. auto.
+    - inversion H0; subst; auto.
+      apply IHis_tree in TREECONT. subst. auto.
+    - inversion H0; subst; auto; rewrite READ0 in READ; inversion READ; subst.
+      apply IHis_tree in TREECONT. subst. auto.
+    - inversion H; subst; auto.
+      rewrite READ0 in READ. inversion READ.
+    - inversion H1; subst; auto.
+      apply IHis_tree1 in ISTREE1. apply IHis_tree2 in ISTREE2. subst. auto.
+    - inversion H0; subst; auto.
+    - inversion H0; subst; auto.
+    - inversion H0; subst; auto.
+      apply IHis_tree in ISTREE1.
+      subst. auto.
+    - inversion H0; subst; auto.
+      destruct plus; discriminate.
+    - inversion H1; subst; auto.
+      + destruct plus; discriminate.
+      + apply plus_one_inj in H4. subst plus0.
+        apply IHis_tree1 in ISTREE1. apply IHis_tree2 in SKIP. subst. auto.
+    - inversion H0; subst; auto.
+      apply IHis_tree in TREECONT. subst. auto.
+    (* Following two bullets copied from backtree repo *)
+    - inversion H1; subst; auto.
+      2: { apply IHis_tree1 in TREELK. subst. exfalso. apply FAIL_LK. auto. }
+      apply IHis_tree1 in TREELK. apply IHis_tree2 in TREECONT. subst. auto.
+    - inversion H0; subst; auto.
+      { apply IHis_tree in TREELK. subst. exfalso. apply FAIL_LK. auto. }
+      apply IHis_tree in TREELK. subst. auto.
+    - inversion H0; subst; auto.
+      + f_equal. auto.
+      + congruence.
+    - inversion H; subst; auto. congruence.
+  Qed.
+
+  Corollary backtree_determ:
+    forall r s t1 t2,
+      backtree r s t1 ->
+      backtree r s t2 ->
+      t1 = t2.
+  Proof.
+    unfold backtree. intros r s t1 t2 H H0. eapply is_tree_determ; eauto.
+  Qed.
+
+  (* We could also prove that there always exists a backtree for any regexes and string,
+   bu that amounts to proving the termination of the backtree construction. *)
+
+
+  (** * Backtracking  *)
+  (* the result of backtracking is just the first branch of the corresponding tree *)
+
+  Inductive backtracking_result: regex -> string -> option leaf -> Prop :=
+  | bt_result:
+    forall r str res tree
+      (TREE: backtree r str tree)
+      (FIRST: first_branch tree = res),
+      backtracking_result r str res.
+
+  Lemma backtracking_determ:
+    forall r str res1 res2,
+      backtracking_result r str res1 ->
+      backtracking_result r str res2 ->
+      res1 = res2.
+  Proof.
+    intros r str res1 res2 H H0. inversion H. subst.
+    inversion H0. subst.
+    specialize (backtree_determ _ _ _ _ TREE TREE0). intros. subst. auto.
+  Qed.
+End Semantics.
