Tree.v
@@ -3,6 +3,7 @@ Import ListNotations.
 
 From Linden Require Import Regex Chars Groups.
 From Coq Require Import PeanoNat.
+From Warblre Require Import Typeclasses Parameters.
 
 
 (* A tree represents all the possible paths that could be explored by a backtracking engine *)
@@ -60,244 +61,249 @@ Inductive groupaction : Type :=
 | Reset (gl:list group_id) (* for capture reset *)
 .
 
-Inductive tree : Type :=
-| Mismatch
-| Match
-| Choice (t1 t2:tree)
-| Read (c:Char) (t:tree)
-| CheckFail (str:string) (* failed to make progress wrt some string *)
-| CheckPass (str:string) (t:tree)
-| GroupAction (g:groupaction) (t: tree)
-| LK (lk: lookaround) (tlk: tree) (t: tree) (* First tree is the lookaround tree. *)
-| LKFail (lk: lookaround) (tlk: tree)
-| AnchorFail (a: anchor)
-| AnchorPass (a: anchor) (t: tree)
-.
 
-(** ** Maximum group ID of a tree *)
-(* Maximum group ID of a list of group IDs *)
-Fixpoint max_gid_list (gl: list group_id) :=
-  match gl with
-  | [] => 0
-  | gid::q => max gid (max_gid_list q)
-  end.
+Section Tree.
+  Context `{characterClass: Character.class}.
+  
+  Inductive tree : Type :=
+  | Mismatch
+  | Match
+  | Choice (t1 t2:tree)
+  | Read (c:Character) (t:tree)
+  | CheckFail (str:string) (* failed to make progress wrt some string *)
+  | CheckPass (str:string) (t:tree)
+  | GroupAction (g:groupaction) (t: tree)
+  | LK (lk: lookaround) (tlk: tree) (t: tree) (* First tree is the lookaround tree. *)
+  | LKFail (lk: lookaround) (tlk: tree)
+  | AnchorFail (a: anchor)
+  | AnchorPass (a: anchor) (t: tree)
+  .
 
-(* Maximum group ID of a groupaction *)
-Definition max_gid_groupaction (act: groupaction) :=
-  match act with
-  | Open gid => gid
-  | Close gid => gid
-  | Reset gl => max_gid_list gl
-  end.
+  (** ** Maximum group ID of a tree *)
+  (* Maximum group ID of a list of group IDs *)
+  Fixpoint max_gid_list (gl: list group_id) :=
+    match gl with
+    | [] => 0
+    | gid::q => max gid (max_gid_list q)
+    end.
 
-(* Maximum group ID of a tree *)
-Fixpoint max_gid_tree (t: tree) :=
-  match t with
-  | Mismatch | Match | CheckFail _ => 0
-  | Choice t1 t2 => max (max_gid_tree t1) (max_gid_tree t2)
-  | Read _ t | CheckPass _ t => max_gid_tree t
-  | GroupAction act t => max (max_gid_groupaction act) (max_gid_tree t)
-  | LK _ tlk t => max (max_gid_tree tlk) (max_gid_tree t)
-  | LKFail _ tlk => max_gid_tree tlk
-  | AnchorFail _ => 0
-  | AnchorPass _ t => max_gid_tree t
-  end.
+  (* Maximum group ID of a groupaction *)
+  Definition max_gid_groupaction (act: groupaction) :=
+    match act with
+    | Open gid => gid
+    | Close gid => gid
+    | Reset gl => max_gid_list gl
+    end.
 
-
-(** * Greedy and Lazy Choice *)
-
-(* a choice operator which depends on the greediness of some quantifier *)
-Definition greedy_choice (greedy:bool) (t1 t2:tree) :=
-  if greedy
-  then Choice t1 t2
-  else Choice t2 t1.
-
-(** * Group action on a group map *)
-Definition group_effect (a: groupaction) (gm: group_map) (idx: nat): group_map :=
-  match a with
-  | Open gid => open_group gm gid idx
-  | Close gid => close_group gm gid idx
-  | Reset gidl => reset_groups gm gidl
-  end.
-
-(** * Tree Results  *)
-
-Definition leaf: Type := (group_map).
-
-(* returning the highest-priority result *)
-(* we also return the corresponding group map *)
-Fixpoint tree_res (t:tree) (gm:group_map) (idx:nat): option leaf :=
-  match t with
-  | Mismatch => None
-  | Match => Some gm
-  | Choice t1 t2 =>
-      seqop (tree_res t1 gm idx) (tree_res t2 gm idx)
-  | Read c t1 => tree_res t1 gm (idx + 1)
-  | CheckFail _ => None
-  | CheckPass _ t1 => tree_res t1 gm idx
-  | GroupAction g t1 => tree_res t1 (group_effect g gm idx) idx
-  | LK lk tlk t1 =>
-      match (positivity lk) with
-      | true => 
-          match tree_res tlk gm idx with
-          | None => None
-          (* using the captures defined in the first branch of the lookahead *)
-          | Some gm' => tree_res t1 gm' idx
-          end
-      | false =>
-          match tree_res tlk gm idx with
-          (* using previous captures *)
-          | None => tree_res t1 gm idx
-          | Some _ => None
-          end
-      end
-  | LKFail _ _ => None
-  | AnchorFail _ => None
-  | AnchorPass _ t => tree_res t gm idx
-  end.
-
-(* initializing on a the empty group map *)
-Definition first_branch (t:tree) : option leaf :=
-  tree_res t empty_group_map 0.
-
-(** * All Tree Results *)
-
-(* returns the ordered list of all results of a tree *)
-(* together with the corresponding group map *)
-Fixpoint tree_leaves (t:tree) (gm:group_map) (idx:nat): list leaf :=
-  match t with
-  | Mismatch => []
-  | Match => [gm]
-  | Choice t1 t2 =>
-      tree_leaves t1 gm idx ++ tree_leaves t2 gm idx
-  | Read c t1 => tree_leaves t1 gm (idx + 1)
-  | CheckFail _ => []
-  | CheckPass _ t1 => tree_leaves t1 gm idx
-  | GroupAction g t1 => tree_leaves t1 (group_effect g gm idx) idx
-  | LK lk tlk t1 =>
-      match (positivity lk) with (* Do we want to explore all the branches of the lookahead tree that succeed? *)
-      | true =>
-          match (tree_leaves tlk gm idx) with
-          | [] => []             (* should not happen *)
-          (* using the captures defined in the first branch of the lookaround *)
-          | gm'::_ => tree_leaves t1 gm' idx
-          end
-      | false =>
-          match (tree_leaves tlk gm idx) with
-          (* using previous captures *)
-          | [] => tree_leaves t1 gm idx
-          | _ => []              (* should not happen *)
-          end
-      end
-  | LKFail _ _ => []
-  | AnchorFail _ => []
-  | AnchorPass _ t => tree_leaves t gm idx
-  end.
+  (* Maximum group ID of a tree *)
+  Fixpoint max_gid_tree (t: tree) :=
+    match t with
+    | Mismatch | Match | CheckFail _ => 0
+    | Choice t1 t2 => max (max_gid_tree t1) (max_gid_tree t2)
+    | Read _ t | CheckPass _ t => max_gid_tree t
+    | GroupAction act t => max (max_gid_groupaction act) (max_gid_tree t)
+    | LK _ tlk t => max (max_gid_tree tlk) (max_gid_tree t)
+    | LKFail _ tlk => max_gid_tree tlk
+    | AnchorFail _ => 0
+    | AnchorPass _ t => max_gid_tree t
+    end.
 
 
-(* Property that this definition coincides on the first element with the previous definition given a tree. *)
-Definition first_tree_leaf_prop (t: tree): Prop :=
-  forall gm idx, tree_res t gm idx = hd_error (tree_leaves t gm idx).
+  (** * Greedy and Lazy Choice *)
+
+  (* a choice operator which depends on the greediness of some quantifier *)
+  Definition greedy_choice (greedy:bool) (t1 t2:tree) :=
+    if greedy
+    then Choice t1 t2
+    else Choice t2 t1.
+
+  (** * Group action on a group map *)
+  Definition group_effect (a: groupaction) (gm: group_map) (idx: nat): group_map :=
+    match a with
+    | Open gid => open_group gm gid idx
+    | Close gid => close_group gm gid idx
+    | Reset gidl => reset_groups gm gidl
+    end.
+
+  (** * Tree Results  *)
+
+  Definition leaf: Type := (group_map).
+
+  (* returning the highest-priority result *)
+  (* we also return the corresponding group map *)
+  Fixpoint tree_res (t:tree) (gm:group_map) (idx:nat): option leaf :=
+    match t with
+    | Mismatch => None
+    | Match => Some gm
+    | Choice t1 t2 =>
+        seqop (tree_res t1 gm idx) (tree_res t2 gm idx)
+    | Read c t1 => tree_res t1 gm (idx + 1)
+    | CheckFail _ => None
+    | CheckPass _ t1 => tree_res t1 gm idx
+    | GroupAction g t1 => tree_res t1 (group_effect g gm idx) idx
+    | LK lk tlk t1 =>
+        match (positivity lk) with
+        | true => 
+            match tree_res tlk gm idx with
+            | None => None
+            (* using the captures defined in the first branch of the lookahead *)
+            | Some gm' => tree_res t1 gm' idx
+            end
+        | false =>
+            match tree_res tlk gm idx with
+            (* using previous captures *)
+            | None => tree_res t1 gm idx
+            | Some _ => None
+            end
+        end
+    | LKFail _ _ => None
+    | AnchorFail _ => None
+    | AnchorPass _ t => tree_res t gm idx
+    end.
+
+  (* initializing on a the empty group map *)
+  Definition first_branch (t:tree) : option leaf :=
+    tree_res t empty_group_map 0.
+
+  (** * All Tree Results *)
+
+  (* returns the ordered list of all results of a tree *)
+  (* together with the corresponding group map *)
+  Fixpoint tree_leaves (t:tree) (gm:group_map) (idx:nat): list leaf :=
+    match t with
+    | Mismatch => []
+    | Match => [gm]
+    | Choice t1 t2 =>
+        tree_leaves t1 gm idx ++ tree_leaves t2 gm idx
+    | Read c t1 => tree_leaves t1 gm (idx + 1)
+    | CheckFail _ => []
+    | CheckPass _ t1 => tree_leaves t1 gm idx
+    | GroupAction g t1 => tree_leaves t1 (group_effect g gm idx) idx
+    | LK lk tlk t1 =>
+        match (positivity lk) with (* Do we want to explore all the branches of the lookahead tree that succeed? *)
+        | true =>
+            match (tree_leaves tlk gm idx) with
+            | [] => []             (* should not happen *)
+            (* using the captures defined in the first branch of the lookaround *)
+            | gm'::_ => tree_leaves t1 gm' idx
+            end
+        | false =>
+            match (tree_leaves tlk gm idx) with
+            (* using previous captures *)
+            | [] => tree_leaves t1 gm idx
+            | _ => []              (* should not happen *)
+            end
+        end
+    | LKFail _ _ => []
+    | AnchorFail _ => []
+    | AnchorPass _ t => tree_leaves t gm idx
+    end.
 
 
-(* intermediate lemma about hd_error *)
-Lemma hd_error_app:
-  forall A (l1 l2:list A),
-    hd_error (l1 ++ l2) =
-      match (hd_error l1) with
-      | Some h => Some h
-      | None => hd_error l2
-      end.
-Proof.
-  intros A l1 l2. induction l1; simpl; auto.
-Qed.
-
-(* Intermediate lemma for positive lookarounds *)
-Lemma first_tree_leaf_poslk:
-  forall lk tlk t1,
-    positivity lk = true -> first_tree_leaf_prop tlk -> first_tree_leaf_prop t1 ->
-    first_tree_leaf_prop (LK lk tlk t1).
-Proof.
-  intros lk tlk t1 Hpos IHtlk IHt1.
-  unfold first_tree_leaf_prop in *. intros gm idx. simpl. rewrite Hpos.
-  specialize (IHtlk gm idx). destruct (tree_res tlk gm idx); destruct (tree_leaves tlk gm idx); try discriminate; simpl in *. 2: reflexivity.
-  injection IHtlk as <-; auto.
-Qed.
-
-(* Intermediate lemma for negative lookarounds *)
-Lemma first_tree_leaf_neglk:
-  forall lk tlk t1,
-    positivity lk = false -> first_tree_leaf_prop tlk -> first_tree_leaf_prop t1 ->
-    first_tree_leaf_prop (LK lk tlk t1).
-Proof.
-  intros lk tlk t1 Hpos IHtlk IHt1.
-  unfold first_tree_leaf_prop in *. intros gm idx. simpl. rewrite Hpos.
-  specialize (IHtlk gm idx). destruct (tree_res tlk gm idx); destruct (tree_leaves tlk gm idx); try discriminate; auto.
-Qed.
+  (* Property that this definition coincides on the first element with the previous definition given a tree. *)
+  Definition first_tree_leaf_prop (t: tree): Prop :=
+    forall gm idx, tree_res t gm idx = hd_error (tree_leaves t gm idx).
 
 
-(* this definition coincides on the first element with the previous definition *)
-Theorem first_tree_leaf:
-  forall t gm idx,
-    tree_res t gm idx = hd_error (tree_leaves t gm idx).
-Proof.
-  intros t. induction t; intros. 1-7,9-11: simpl; auto.
-  - rewrite IHt1. rewrite IHt2. rewrite hd_error_app. unfold seqop.
-    destruct (hd_error (tree_leaves t1 gm idx)) eqn:HD; auto.
-  - destruct (positivity lk) eqn:Hlkpos. + now apply first_tree_leaf_poslk. + now apply first_tree_leaf_neglk.
-Qed.
-      
-(** * Group Map irrelevance  *)
-(* finding a match does not depend on the initial group map *)
-(* we could phrase a stronger theorem about how to relate the two results *)
-(* but for now I only need to differentiate when there is no results from when there is one *)
+  (* intermediate lemma about hd_error *)
+  Lemma hd_error_app:
+    forall A (l1 l2:list A),
+      hd_error (l1 ++ l2) =
+        match (hd_error l1) with
+        | Some h => Some h
+        | None => hd_error l2
+        end.
+  Proof.
+    intros A l1 l2. induction l1; simpl; auto.
+  Qed.
 
-(* warning: actually so far I don't need this theorem *)
+  (* Intermediate lemma for positive lookarounds *)
+  Lemma first_tree_leaf_poslk:
+    forall lk tlk t1,
+      positivity lk = true -> first_tree_leaf_prop tlk -> first_tree_leaf_prop t1 ->
+      first_tree_leaf_prop (LK lk tlk t1).
+  Proof.
+    intros lk tlk t1 Hpos IHtlk IHt1.
+    unfold first_tree_leaf_prop in *. intros gm idx. simpl. rewrite Hpos.
+    specialize (IHtlk gm idx). destruct (tree_res tlk gm idx); destruct (tree_leaves tlk gm idx); try discriminate; simpl in *. 2: reflexivity.
+    injection IHtlk as <-; auto.
+  Qed.
 
-(* Group map irrelevance property for a given tree. *)
-Definition leaves_group_map_indep_prop (t: tree): Prop :=
-  forall gm1 gm2 idx1 idx2,
-    tree_leaves t gm1 idx1 = [] -> tree_leaves t gm2 idx2 = [].
-
-(* Intermediate lemma for positive lookarounds *)
-Lemma leaves_group_map_indep_poslk:
-  forall lk tlk t1,
-    positivity lk = true -> leaves_group_map_indep_prop tlk -> leaves_group_map_indep_prop t1 ->
-    leaves_group_map_indep_prop (LK lk tlk t1).
-Proof.
-  intros lk tlk t1 Hposlk IHtlk IHt1; unfold leaves_group_map_indep_prop in *; simpl.
-  rewrite Hposlk. intros gm1 gm2 idx1 idx2 Hnil1.
-  specialize (IHtlk gm1 gm2 idx1 idx2). destruct (tree_leaves tlk gm1 idx1) as [|gm' q]; simpl in *.
-  1: { specialize (IHtlk eq_refl). now rewrite IHtlk. }
-  destruct (tree_leaves tlk gm2 idx2) as [|gm'0 q0]; simpl in *. 1: reflexivity.
-  eapply IHt1; eauto.
-Qed.
-
-(* Intermediate lemma for negative lookarounds *)
-Lemma leaves_group_map_indep_neglk:
-  forall lk tlk t1,
-    positivity lk = false -> leaves_group_map_indep_prop tlk -> leaves_group_map_indep_prop t1 ->
-    leaves_group_map_indep_prop (LK lk tlk t1).
-Proof.
-  intros lk tlk t1 Hposlk IHtlk IHt1; unfold leaves_group_map_indep_prop in *; simpl.
-  rewrite Hposlk. intros gm1 gm2 idx1 idx2 Hnil1.
-  destruct (tree_leaves tlk gm1 idx1) as [|gm' q] eqn:Hnilsub1; simpl in *.
-  1: { specialize (IHtlk gm1 gm2 idx1 idx2 Hnilsub1). rewrite IHtlk. eapply IHt1; eauto. }
-  destruct (tree_leaves tlk gm2 idx2) as [|gm'0 q0] eqn:Hnilsub2; simpl in *. 2: reflexivity.
-  exfalso. apply IHtlk with (gm2 := gm1) (idx2 := idx1) in Hnilsub2. congruence.
-Qed.
+  (* Intermediate lemma for negative lookarounds *)
+  Lemma first_tree_leaf_neglk:
+    forall lk tlk t1,
+      positivity lk = false -> first_tree_leaf_prop tlk -> first_tree_leaf_prop t1 ->
+      first_tree_leaf_prop (LK lk tlk t1).
+  Proof.
+    intros lk tlk t1 Hpos IHtlk IHt1.
+    unfold first_tree_leaf_prop in *. intros gm idx. simpl. rewrite Hpos.
+    specialize (IHtlk gm idx). destruct (tree_res tlk gm idx); destruct (tree_leaves tlk gm idx); try discriminate; auto.
+  Qed.
 
 
-Lemma leaves_group_map_indep:
-  forall t gm1 gm2 idx1 idx2,
-    tree_leaves t gm1 idx1 = [] -> tree_leaves t gm2 idx2 = [].
-Proof.
-  intros t.
-  induction t; intros. 1-7,9-11: simpl; auto;
-    simpl in H; try solve[inversion H];
-    try solve[eapply IHt in H; eauto].
-  - apply app_eq_nil in H as [NIL1 NIL2].
-    apply IHt1 with (gm2:=gm2) (idx2:=idx2) in NIL1. apply IHt2 with (gm2:=gm2) (idx2:=idx2) in NIL2.
-    rewrite NIL1. rewrite NIL2. auto.
-  - destruct (positivity lk) eqn:Hlkpos. + eapply leaves_group_map_indep_poslk; eauto. + eapply leaves_group_map_indep_neglk; eauto.
-Qed.
+  (* this definition coincides on the first element with the previous definition *)
+  Theorem first_tree_leaf:
+    forall t gm idx,
+      tree_res t gm idx = hd_error (tree_leaves t gm idx).
+  Proof.
+    intros t. induction t; intros. 1-7,9-11: simpl; auto.
+    - rewrite IHt1. rewrite IHt2. rewrite hd_error_app. unfold seqop.
+      destruct (hd_error (tree_leaves t1 gm idx)) eqn:HD; auto.
+    - destruct (positivity lk) eqn:Hlkpos. + now apply first_tree_leaf_poslk. + now apply first_tree_leaf_neglk.
+  Qed.
+
+  (** * Group Map irrelevance  *)
+  (* finding a match does not depend on the initial group map *)
+  (* we could phrase a stronger theorem about how to relate the two results *)
+  (* but for now I only need to differentiate when there is no results from when there is one *)
+
+  (* warning: actually so far I don't need this theorem *)
+
+  (* Group map irrelevance property for a given tree. *)
+  Definition leaves_group_map_indep_prop (t: tree): Prop :=
+    forall gm1 gm2 idx1 idx2,
+      tree_leaves t gm1 idx1 = [] -> tree_leaves t gm2 idx2 = [].
+
+  (* Intermediate lemma for positive lookarounds *)
+  Lemma leaves_group_map_indep_poslk:
+    forall lk tlk t1,
+      positivity lk = true -> leaves_group_map_indep_prop tlk -> leaves_group_map_indep_prop t1 ->
+      leaves_group_map_indep_prop (LK lk tlk t1).
+  Proof.
+    intros lk tlk t1 Hposlk IHtlk IHt1; unfold leaves_group_map_indep_prop in *; simpl.
+    rewrite Hposlk. intros gm1 gm2 idx1 idx2 Hnil1.
+    specialize (IHtlk gm1 gm2 idx1 idx2). destruct (tree_leaves tlk gm1 idx1) as [|gm' q]; simpl in *.
+    1: { specialize (IHtlk eq_refl). now rewrite IHtlk. }
+    destruct (tree_leaves tlk gm2 idx2) as [|gm'0 q0]; simpl in *. 1: reflexivity.
+    eapply IHt1; eauto.
+  Qed.
+
+  (* Intermediate lemma for negative lookarounds *)
+  Lemma leaves_group_map_indep_neglk:
+    forall lk tlk t1,
+      positivity lk = false -> leaves_group_map_indep_prop tlk -> leaves_group_map_indep_prop t1 ->
+      leaves_group_map_indep_prop (LK lk tlk t1).
+  Proof.
+    intros lk tlk t1 Hposlk IHtlk IHt1; unfold leaves_group_map_indep_prop in *; simpl.
+    rewrite Hposlk. intros gm1 gm2 idx1 idx2 Hnil1.
+    destruct (tree_leaves tlk gm1 idx1) as [|gm' q] eqn:Hnilsub1; simpl in *.
+    1: { specialize (IHtlk gm1 gm2 idx1 idx2 Hnilsub1). rewrite IHtlk. eapply IHt1; eauto. }
+    destruct (tree_leaves tlk gm2 idx2) as [|gm'0 q0] eqn:Hnilsub2; simpl in *. 2: reflexivity.
+    exfalso. apply IHtlk with (gm2 := gm1) (idx2 := idx1) in Hnilsub2. congruence.
+  Qed.
+
+
+  Lemma leaves_group_map_indep:
+    forall t gm1 gm2 idx1 idx2,
+      tree_leaves t gm1 idx1 = [] -> tree_leaves t gm2 idx2 = [].
+  Proof.
+    intros t.
+    induction t; intros. 1-7,9-11: simpl; auto;
+      simpl in H; try solve[inversion H];
+      try solve[eapply IHt in H; eauto].
+    - apply app_eq_nil in H as [NIL1 NIL2].
+      apply IHt1 with (gm2:=gm2) (idx2:=idx2) in NIL1. apply IHt2 with (gm2:=gm2) (idx2:=idx2) in NIL2.
+      rewrite NIL1. rewrite NIL2. auto.
+    - destruct (positivity lk) eqn:Hlkpos. + eapply leaves_group_map_indep_poslk; eauto. + eapply leaves_group_map_indep_neglk; eauto.
+  Qed.
+End Tree.
