warblreequiv/CharDescrCharSet.v
@@ -5,189 +5,194 @@ Import Patterns.
 
 Local Open Scope result_flow.
 
-Definition equiv_cd_charset (cd: char_descr) (charset: CharSet) :=
-  forall c: Chars.Char, char_match c cd = CharSet.contains charset c.
-
-(* Lemma for character descriptor inversion *)
-Lemma equiv_cd_inv:
-  forall cd s, equiv_cd_charset cd s -> equiv_cd_charset (CdInv cd) (CharSet.remove_all Characters.all s).
-Proof.
-  intros cd s H c.
-  rewrite charset_remove_all_contains. simpl. specialize (H c).
-  unfold Characters.all, Character.all. simpl. rewrite charset_from_list_contains_inb, char_all_inb. simpl. now f_equal.
-Qed.
-
-(* Lemma for character descriptor union *)
-Lemma equiv_cd_union:
-  forall cd1 cd2 s1 s2,
-    equiv_cd_charset cd1 s1 -> equiv_cd_charset cd2 s2 ->
-    equiv_cd_charset (CdUnion cd1 cd2) (CharSet.union s1 s2).
-Proof.
-  intros cd1 cd2 s1 s2 Hequiv1 Hequiv2 c.
-  simpl. rewrite charset_union_contains. rewrite Hequiv1. rewrite Hequiv2. reflexivity.
-Qed.
-
-(* Inversion lemma for singletons *)
-Lemma equiv_cd_singleton_invn:
-  forall c s,
-    equiv_cd_charset (CdSingle c) s -> s = CharSet.singleton c.
-Proof.
-  intros c s Hequiv. apply charset_ext. intro chr.
-  specialize (Hequiv chr). simpl in Hequiv.
-  setoid_rewrite <- Hequiv. symmetry. apply charset_contains_singleton.
-Qed.
-
-(* Lemmas for various character descriptors *)
-Lemma equiv_cd_empty:
-  equiv_cd_charset CdEmpty CharSet.empty.
-Proof.
-  intro c. simpl. rewrite charset_empty_contains. reflexivity.
-Qed.
-
-Lemma equiv_cd_digits:
-  equiv_cd_charset CdDigits Characters.digits.
-Proof.
-  intro c. simpl. unfold Characters.digits. now rewrite charset_from_list_contains_inb.
-Qed.
-
-Lemma equiv_cd_whitespace:
-  equiv_cd_charset CdWhitespace (CharSet.union Characters.white_spaces Characters.line_terminators).
-Proof.
-  intro c. simpl. unfold Characters.white_spaces, Characters.line_terminators. rewrite charset_union_contains. now do 2 rewrite charset_from_list_contains_inb.
-Qed.
-
-Lemma equiv_cd_wordchar:
-  equiv_cd_charset CdWordChar Characters.ascii_word_characters.
-Proof.
-  intro c. simpl. unfold Characters.ascii_word_characters. now rewrite charset_from_list_contains_inb.
-Qed.
-
-Lemma equiv_cd_range:
-  forall cl ch,
-    char_numeric_value cl <= char_numeric_value ch ->
-    equiv_cd_charset (CdRange cl ch) (CharSet.range cl ch).
-Proof.
-  intros cl ch Hle c. simpl.
-  admit. (* Missing axiom? *)
-Admitted.
-
-(* TODO Take dotAll flag into account *)
-Lemma equiv_cd_dot:
-  equiv_cd_charset CdDot Characters.all.
-Proof.
-  intro c. simpl. unfold Characters.all, Character.all. simpl.
-  rewrite charset_from_list_contains_inb. symmetry. apply char_all_inb.
-Qed.
-
-Lemma equiv_cd_single:
-  forall c, equiv_cd_charset (CdSingle c) (CharSet.singleton c).
-Proof.
-  intros c chr. simpl. symmetry. apply charset_contains_singleton.
-Qed.
-
-(* Lemma for CharacterClassEscapes *)
-Lemma equiv_cd_CharacterClassEscape:
-  forall esc cd rer,
-    RegExpRecord.ignoreCase rer = false ->
-    equiv_CharacterClassEscape esc cd ->
-    exists a, Semantics.compileToCharSet_ClassAtom (ClassEsc (CCharacterClassEsc esc)) rer = Success a /\
-           equiv_cd_charset cd a.
-Proof.
-  intros esc cd rer Hcasesenst Hequiv.
-  inversion Hequiv as [Heqesc Heqcd | Heqesc Heqcd | Heqesc Heqcd | Heqesc Heqcd | Heqesc Heqcd | Heqesc Heqcd]; simpl; unfold Coercions.Coercions.wrap_CharSet; eexists; split; try solve[reflexivity].
-  - apply equiv_cd_digits.
-  - apply equiv_cd_inv. apply equiv_cd_digits.
-  - apply equiv_cd_whitespace.
-  - apply equiv_cd_inv. apply equiv_cd_whitespace.
-  - pose proof wordCharacters_casesenst rer Hcasesenst. unfold Semantics.wordCharacters, Coercions.Coercions.wrap_CharSet in H. simpl in H. injection H as H. setoid_rewrite H. apply equiv_cd_wordchar.
-  - apply equiv_cd_inv. pose proof wordCharacters_casesenst rer Hcasesenst. unfold Semantics.wordCharacters, Coercions.Coercions.wrap_CharSet in H. simpl in H. injection H as H. setoid_rewrite H. apply equiv_cd_wordchar.
-Qed.
-
-(* Lemma for ControlEscapes *)
-Lemma equiv_cd_ControlEscape:
-  forall esc cd rer,
-    equiv_ControlEscape esc cd ->
-    exists a, Semantics.compileToCharSet_ClassAtom (ClassEsc (CCharacterEsc (ControlEsc esc))) rer = Success a /\
-           equiv_cd_charset cd a.
-Proof.
-  intros esc cd rer Hequiv.
-  inversion Hequiv; simpl; unfold Coercions.Coercions.wrap_CharSet; eexists; split; try solve[reflexivity]; unfold Numeric.nat_to_nni; rewrite char_numeric_pseudo_bij; apply equiv_cd_single.
-Qed.
-
-(* Lemma for CharacterEscapes *)
-Lemma equiv_cd_CharacterEscape:
-  forall esc cd rer,
-    equiv_CharacterEscape esc cd ->
-    exists a, Semantics.compileToCharSet_ClassAtom (ClassEsc (CCharacterEsc esc)) rer = Success a /\
-           equiv_cd_charset cd a.
-Proof.
-  intros esc cd rer Hequiv. inversion Hequiv as [esc0 cd0 Hequiv' Heqesc Heqcd0 | l cd0 Hequiv' Heqesc Heqcd0 | Heqesc Heqcd].
-  - apply equiv_cd_ControlEscape. assumption.
-  - admit. (* AsciiControlEsc *)
-  - simpl. unfold Coercions.Coercions.wrap_CharSet. eexists. split. 1: reflexivity.
-    unfold Numeric.nat_to_nni. rewrite char_numeric_pseudo_bij. apply equiv_cd_single.
-Admitted.
-
-(* Lemma for ClassEscapes *)
-Lemma equiv_cd_ClassEscape:
-  forall esc cd rer,
-    RegExpRecord.ignoreCase rer = false ->
-    equiv_ClassEscape esc cd ->
-    exists a, Semantics.compileToCharSet_ClassAtom (ClassEsc esc) rer = Success a /\
-           equiv_cd_charset cd a.
-Proof.
-  intros esc cd rer Hcasesenst Hequiv. inversion Hequiv as [Heqesc Heqcd | Heqesc Heqcd | |].
-  - simpl. unfold Coercions.Coercions.wrap_CharSet. eexists. split.
-    + reflexivity.
-    + unfold Numeric.nat_to_nni. rewrite char_numeric_pseudo_bij. apply equiv_cd_single.
-  - simpl. unfold Coercions.Coercions.wrap_CharSet. eexists. split.
-    + reflexivity.
-    + unfold Numeric.nat_to_nni. rewrite char_numeric_pseudo_bij. apply equiv_cd_single.
-  - apply equiv_cd_CharacterClassEscape; auto.
-  - apply equiv_cd_CharacterEscape; auto.
-Qed.
-
-(* Lemmas for ClassRanges *)
-Lemma equiv_cd_ClassAtom:
-  forall ca cacd rer,
-    RegExpRecord.ignoreCase rer = false ->
-    equiv_ClassAtom ca cacd ->
-    exists a, Semantics.compileToCharSet_ClassAtom ca rer = Success a /\ equiv_cd_charset cacd a.
-Proof.
-  intros ca cacd rer Hcasesenst Hequiv.
-  inversion Hequiv as [c Heqca Heqcacd | esc cd Hequiv' Heqca Heqcacd].
-  - simpl. unfold Coercions.Coercions.wrap_CharSet. eexists. split. + reflexivity. + apply equiv_cd_single.
-  - apply equiv_cd_ClassEscape; assumption.
-Qed.
+Section CharDescrCharSet.
+  Context `{characterClass: Character.class}.
   
+  Definition equiv_cd_charset (cd: char_descr) (charset: CharSet) :=
+    forall c: Character, char_match c cd = CharSet.contains charset c.
 
-Lemma equiv_cd_ClassRanges:
-  forall crs cd rer,
-    RegExpRecord.ignoreCase rer = false ->
-    equiv_ClassRanges crs cd ->
-    exists a, Semantics.compileToCharSet crs rer = Success a /\
-           equiv_cd_charset cd a.
-Proof.
-  intros crs cd rer Hcasesenst Hequiv.
-  induction Hequiv as [|ca cacd t tcd Hequiv' Hequiv IH | l h cl ch t tcd Hequivl Hequivh Hl_le_h Hequiv IH].
-  - simpl. unfold Coercions.Coercions.wrap_CharSet.
-    eexists. split. + reflexivity. + apply equiv_cd_empty.
-  - simpl. pose proof equiv_cd_ClassAtom ca cacd rer Hcasesenst Hequiv' as [A [HeqA Hequivatom]].
-    rewrite HeqA. simpl.
-    destruct IH as [B [HeqB IH]]. rewrite HeqB. simpl.
-    unfold Coercions.Coercions.wrap_CharSet. eexists. split. + reflexivity. + now apply equiv_cd_union.
-  - simpl.
-    pose proof equiv_cd_ClassAtom l (CdSingle cl) rer Hcasesenst Hequivl as [A [HeqA Hequivatoml]].
-    pose proof equiv_cd_ClassAtom h (CdSingle ch) rer Hcasesenst Hequivh as [B [HeqB Hequivatomh]].
-    rewrite HeqA, HeqB. simpl.
-    destruct IH as [C [HeqC IH]]. rewrite HeqC. simpl.
-    unfold Semantics.characterRange.
-    pose proof equiv_cd_singleton_invn cl A Hequivatoml as HAsingleton.
-    pose proof equiv_cd_singleton_invn ch B Hequivatomh as HBsingleton.
-    rewrite HAsingleton, HBsingleton. do 2 rewrite CharSet.singleton_size. simpl.
-    do 2 rewrite CharSet.singleton_unique. simpl.
-    pose proof Hl_le_h as Hl_le_h'. rewrite <- PeanoNat.Nat.leb_le in Hl_le_h'. rewrite Hl_le_h'. simpl.
-    unfold Coercions.Coercions.wrap_CharSet. eexists. split.
-    + reflexivity.
-    + apply equiv_cd_union; auto. do 2 rewrite char_numeric_pseudo_bij. apply equiv_cd_range. assumption.
-Qed.
+  (* Lemma for character descriptor inversion *)
+  Lemma equiv_cd_inv:
+    forall cd s, equiv_cd_charset cd s -> equiv_cd_charset (CdInv cd) (CharSet.remove_all Characters.all s).
+  Proof.
+    intros cd s H c.
+    rewrite charset_remove_all_contains. simpl. specialize (H c).
+    unfold Characters.all, Character.all. simpl. setoid_rewrite charset_from_list_contains_inb. setoid_rewrite char_all_inb. simpl. now f_equal.
+  Qed.
+
+  (* Lemma for character descriptor union *)
+  Lemma equiv_cd_union:
+    forall cd1 cd2 s1 s2,
+      equiv_cd_charset cd1 s1 -> equiv_cd_charset cd2 s2 ->
+      equiv_cd_charset (CdUnion cd1 cd2) (CharSet.union s1 s2).
+  Proof.
+    intros cd1 cd2 s1 s2 Hequiv1 Hequiv2 c.
+    simpl. setoid_rewrite charset_union_contains. rewrite Hequiv1. rewrite Hequiv2. reflexivity.
+  Qed.
+
+  (* Inversion lemma for singletons *)
+  Lemma equiv_cd_singleton_invn:
+    forall c s,
+      equiv_cd_charset (CdSingle c) s -> s = CharSet.singleton c.
+  Proof.
+    intros c s Hequiv. apply charset_ext. intro chr.
+    specialize (Hequiv chr). simpl in Hequiv.
+    setoid_rewrite <- Hequiv. symmetry. apply charset_contains_singleton.
+  Qed.
+
+  (* Lemmas for various character descriptors *)
+  Lemma equiv_cd_empty:
+    equiv_cd_charset CdEmpty CharSet.empty.
+  Proof.
+    intro c. simpl. setoid_rewrite charset_empty_contains. reflexivity.
+  Qed.
+
+  Lemma equiv_cd_digits:
+    equiv_cd_charset CdDigits Characters.digits.
+  Proof.
+    intro c. simpl. unfold Characters.digits. now setoid_rewrite charset_from_list_contains_inb.
+  Qed.
+
+  Lemma equiv_cd_whitespace:
+    equiv_cd_charset CdWhitespace (CharSet.union Characters.white_spaces Characters.line_terminators).
+  Proof.
+    intro c. simpl. unfold Characters.white_spaces, Characters.line_terminators. setoid_rewrite charset_union_contains. now do 2 rewrite charset_from_list_contains_inb.
+  Qed.
+
+  Lemma equiv_cd_wordchar:
+    equiv_cd_charset CdWordChar Characters.ascii_word_characters.
+  Proof.
+    intro c. simpl. unfold Characters.ascii_word_characters. now setoid_rewrite charset_from_list_contains_inb.
+  Qed.
+
+  Lemma equiv_cd_range:
+    forall cl ch,
+      Character.numeric_value cl <= Character.numeric_value ch ->
+      equiv_cd_charset (CdRange cl ch) (CharSet.range cl ch).
+  Proof.
+    intros cl ch Hle c. simpl.
+
+    admit. (* Missing axiom? *)
+  Admitted.
+
+  (* TODO Take dotAll flag into account *)
+  Lemma equiv_cd_dot:
+    equiv_cd_charset CdDot Characters.all.
+  Proof.
+    intro c. simpl. unfold Characters.all, Character.all. simpl.
+    setoid_rewrite charset_from_list_contains_inb. symmetry. apply char_all_inb.
+  Qed.
+
+  Lemma equiv_cd_single:
+    forall c, equiv_cd_charset (CdSingle c) (CharSet.singleton c).
+  Proof.
+    intros c chr. simpl. symmetry. apply charset_contains_singleton.
+  Qed.
+
+  (* Lemma for CharacterClassEscapes *)
+  Lemma equiv_cd_CharacterClassEscape:
+    forall esc cd rer,
+      RegExpRecord.ignoreCase rer = false ->
+      equiv_CharacterClassEscape esc cd ->
+      exists a, Semantics.compileToCharSet_ClassAtom (ClassEsc (CCharacterClassEsc esc)) rer = Success a /\
+             equiv_cd_charset cd a.
+  Proof.
+    intros esc cd rer Hcasesenst Hequiv.
+    inversion Hequiv as [Heqesc Heqcd | Heqesc Heqcd | Heqesc Heqcd | Heqesc Heqcd | Heqesc Heqcd | Heqesc Heqcd]; simpl; unfold Coercions.Coercions.wrap_CharSet; eexists; split; try solve[reflexivity].
+    - apply equiv_cd_digits.
+    - apply equiv_cd_inv. apply equiv_cd_digits.
+    - apply equiv_cd_whitespace.
+    - apply equiv_cd_inv. apply equiv_cd_whitespace.
+    - pose proof wordCharacters_casesenst rer Hcasesenst. unfold Semantics.wordCharacters, Coercions.Coercions.wrap_CharSet in H. simpl in H. injection H as H. setoid_rewrite H. apply equiv_cd_wordchar.
+    - apply equiv_cd_inv. pose proof wordCharacters_casesenst rer Hcasesenst. unfold Semantics.wordCharacters, Coercions.Coercions.wrap_CharSet in H. simpl in H. injection H as H. setoid_rewrite H. apply equiv_cd_wordchar.
+  Qed.
+
+  (* Lemma for ControlEscapes *)
+  Lemma equiv_cd_ControlEscape:
+    forall esc cd rer,
+      equiv_ControlEscape esc cd ->
+      exists a, Semantics.compileToCharSet_ClassAtom (ClassEsc (CCharacterEsc (ControlEsc esc))) rer = Success a /\
+             equiv_cd_charset cd a.
+  Proof.
+    intros esc cd rer Hequiv.
+    inversion Hequiv; simpl; unfold Coercions.Coercions.wrap_CharSet; eexists; split; try solve[reflexivity]; unfold Numeric.nat_to_nni; rewrite Character.numeric_pseudo_bij; apply equiv_cd_single.
+  Qed.
+
+  (* Lemma for CharacterEscapes *)
+  Lemma equiv_cd_CharacterEscape:
+    forall esc cd rer,
+      equiv_CharacterEscape esc cd ->
+      exists a, Semantics.compileToCharSet_ClassAtom (ClassEsc (CCharacterEsc esc)) rer = Success a /\
+             equiv_cd_charset cd a.
+  Proof.
+    intros esc cd rer Hequiv. inversion Hequiv as [esc0 cd0 Hequiv' Heqesc Heqcd0 | l cd0 Hequiv' Heqesc Heqcd0 | Heqesc Heqcd].
+    - apply equiv_cd_ControlEscape. assumption.
+    - admit. (* AsciiControlEsc *)
+    - simpl. unfold Coercions.Coercions.wrap_CharSet. eexists. split. 1: reflexivity.
+      unfold Numeric.nat_to_nni. rewrite Character.numeric_pseudo_bij. apply equiv_cd_single.
+  Admitted.
+
+  (* Lemma for ClassEscapes *)
+  Lemma equiv_cd_ClassEscape:
+    forall esc cd rer,
+      RegExpRecord.ignoreCase rer = false ->
+      equiv_ClassEscape esc cd ->
+      exists a, Semantics.compileToCharSet_ClassAtom (ClassEsc esc) rer = Success a /\
+             equiv_cd_charset cd a.
+  Proof.
+    intros esc cd rer Hcasesenst Hequiv. inversion Hequiv as [Heqesc Heqcd | Heqesc Heqcd | |].
+    - simpl. unfold Coercions.Coercions.wrap_CharSet. eexists. split.
+      + reflexivity.
+      + unfold Numeric.nat_to_nni. rewrite Character.numeric_pseudo_bij. apply equiv_cd_single.
+    - simpl. unfold Coercions.Coercions.wrap_CharSet. eexists. split.
+      + reflexivity.
+      + unfold Numeric.nat_to_nni. rewrite Character.numeric_pseudo_bij. apply equiv_cd_single.
+    - apply equiv_cd_CharacterClassEscape; auto.
+    - apply equiv_cd_CharacterEscape; auto.
+  Qed.
+
+  (* Lemmas for ClassRanges *)
+  Lemma equiv_cd_ClassAtom:
+    forall ca cacd rer,
+      RegExpRecord.ignoreCase rer = false ->
+      equiv_ClassAtom ca cacd ->
+      exists a, Semantics.compileToCharSet_ClassAtom ca rer = Success a /\ equiv_cd_charset cacd a.
+  Proof.
+    intros ca cacd rer Hcasesenst Hequiv.
+    inversion Hequiv as [c Heqca Heqcacd | esc cd Hequiv' Heqca Heqcacd].
+    - simpl. unfold Coercions.Coercions.wrap_CharSet. eexists. split. + reflexivity. + apply equiv_cd_single.
+    - apply equiv_cd_ClassEscape; assumption.
+  Qed.
+
+
+  Lemma equiv_cd_ClassRanges:
+    forall crs cd rer,
+      RegExpRecord.ignoreCase rer = false ->
+      equiv_ClassRanges crs cd ->
+      exists a, Semantics.compileToCharSet crs rer = Success a /\
+             equiv_cd_charset cd a.
+  Proof.
+    intros crs cd rer Hcasesenst Hequiv.
+    induction Hequiv as [|ca cacd t tcd Hequiv' Hequiv IH | l h cl ch t tcd Hequivl Hequivh Hl_le_h Hequiv IH].
+    - simpl. unfold Coercions.Coercions.wrap_CharSet.
+      eexists. split. + reflexivity. + apply equiv_cd_empty.
+    - simpl. pose proof equiv_cd_ClassAtom ca cacd rer Hcasesenst Hequiv' as [A [HeqA Hequivatom]].
+      rewrite HeqA. simpl.
+      destruct IH as [B [HeqB IH]]. rewrite HeqB. simpl.
+      unfold Coercions.Coercions.wrap_CharSet. eexists. split. + reflexivity. + now apply equiv_cd_union.
+    - simpl.
+      pose proof equiv_cd_ClassAtom l (CdSingle cl) rer Hcasesenst Hequivl as [A [HeqA Hequivatoml]].
+      pose proof equiv_cd_ClassAtom h (CdSingle ch) rer Hcasesenst Hequivh as [B [HeqB Hequivatomh]].
+      rewrite HeqA, HeqB. simpl.
+      destruct IH as [C [HeqC IH]]. rewrite HeqC. simpl.
+      unfold Semantics.characterRange.
+      pose proof equiv_cd_singleton_invn cl A Hequivatoml as HAsingleton.
+      pose proof equiv_cd_singleton_invn ch B Hequivatomh as HBsingleton.
+      rewrite HAsingleton, HBsingleton. do 2 rewrite CharSet.singleton_size. simpl.
+      do 2 rewrite CharSet.singleton_unique. simpl.
+      pose proof Hl_le_h as Hl_le_h'. rewrite <- PeanoNat.Nat.leb_le in Hl_le_h'. rewrite Hl_le_h'. simpl.
+      unfold Coercions.Coercions.wrap_CharSet. eexists. split.
+      + reflexivity.
+      + apply equiv_cd_union; auto. do 2 rewrite Character.numeric_pseudo_bij. apply equiv_cd_range. assumption.
+  Qed.
+End CharDescrCharSet.
