warblreequiv/LWEquivMain.v
@@ -12,48 +12,51 @@ Local Open Scope result_flow.
 
 (** * Main equivalence theorem *)
 
+Section LWEquivMain.
+  Context `{characterClass: Character.class}.
+  
+  (* The main theorem *)
+  Theorem linden_warblre_equiv:
+    forall (wreg: Patterns.Regex) (lreg: regex) (str: string) (rer: RegExpRecord)
+      (matcher: string -> non_neg_integer -> MatchResult)
+      (tmatcher: string -> non_neg_integer -> TMatchResult)
+      (res: MatchResult) (tres: TMatchResult) (t: tree),
+      RegExpRecord.ignoreCase rer = false ->
+      RegExpRecord.multiline rer = false ->
+      RegExpRecord.dotAll rer = true ->
+      RegExpRecord.capturingGroupsCount rer = StaticSemantics.countLeftCapturingParensWithin wreg [] ->
+      (* For all pairs of equivalent Warblre and Linden regexes wreg and lreg, *)
+      equiv_regex wreg lreg ->
+      (* if the compilations of these regexes both succeed, *)
+      Semantics.compilePattern wreg rer = Success matcher ->
+      tCompilePattern wreg rer = Success tmatcher ->
+      (* letting res and tres be the respective results of these matchers on some input string str, *)
+      res = matcher str 0 -> tres = tmatcher str 0 ->
+      (* these results define the same capture groups if both matchings succeed and *)
+      LWEquivTMatcherDef.equiv_results tres (MatchState.init rer str 0) [] forward res /\
+        (* in this case, the backtree of the tree matcher respects the relational semantics. *)
+        (tres = Success t -> is_tree lreg [] (init_input str) forward t).
+  Proof.
+    intros wreg lreg str rer matcher tmatcher res tres t Hcasesenst Hnomultiline HdotAll Hcapcount Hequiv.
+    unfold Semantics.compilePattern, tCompilePattern.
 
-(* The main theorem *)
-Theorem linden_warblre_equiv:
-  forall (wreg: Patterns.Regex) (lreg: regex) (str: string) (rer: RegExpRecord)
-    (matcher: string -> non_neg_integer -> MatchResult)
-    (tmatcher: string -> non_neg_integer -> TMatchResult)
-    (res: MatchResult) (tres: TMatchResult) (t: tree),
-    RegExpRecord.ignoreCase rer = false ->
-    RegExpRecord.multiline rer = false ->
-    RegExpRecord.dotAll rer = true ->
-    RegExpRecord.capturingGroupsCount rer = StaticSemantics.countLeftCapturingParensWithin wreg [] ->
-    (* For all pairs of equivalent Warblre and Linden regexes wreg and lreg, *)
-    equiv_regex wreg lreg ->
-    (* if the compilations of these regexes both succeed, *)
-    Semantics.compilePattern wreg rer = Success matcher ->
-    tCompilePattern wreg rer = Success tmatcher ->
-    (* letting res and tres be the respective results of these matchers on some input string str, *)
-    res = matcher str 0 -> tres = tmatcher str 0 ->
-    (* these results define the same capture groups if both matchings succeed and *)
-    LWEquivTMatcherDef.equiv_results tres (MatchState.init rer str 0) [] forward res /\
-      (* in this case, the backtree of the tree matcher respects the relational semantics. *)
-      (tres = Success t -> is_tree lreg [] (init_input str) forward t).
-Proof.
-  intros wreg lreg str rer matcher tmatcher res tres t Hcasesenst Hnomultiline HdotAll Hcapcount Hequiv.
-  unfold Semantics.compilePattern, tCompilePattern.
-  
-  pose proof compile_tcompile wreg [] rer as Hcompile_tcompile.
-  pose proof tmatcher_bt rer lreg wreg Hcasesenst Hnomultiline HdotAll Hequiv wreg lreg [] as Hbt.
-  specialize_prove Hbt by constructor. specialize (Hbt Hequiv).
-  
-  destruct Semantics.compileSubPattern as [m|] eqn:Heqm; simpl. 2: discriminate.
-  destruct tCompileSubPattern as [tm|] eqn:Heqtm; simpl. 2: discriminate.
-  specialize (Hcompile_tcompile m tm forward Heqm Heqtm str).
-  specialize (Hbt tm forward Heqtm).
-  intros Heqmatcher Heqtmatcher. injection Heqmatcher as <-. injection Heqtmatcher as <-.
-  intros Heqres Heqtres. subst res tres.
-  destruct negb. (* Negative length! *) 1: { split. - constructor. - discriminate. }
-  split.
-  - apply Hcompile_tcompile. + apply id_equiv. + reflexivity.
-  - specialize (Hbt id_tmcont [] str (id_tmcont_valid rer str forward)).
-    specialize (Hbt (init_input str) (MSInput.init_input_compat str)).
-    set (ms := match_state str 0 _). specialize (Hbt ms t).
-    specialize_prove Hbt by apply MSInput.init_ms_matches_inp. simpl in Hbt.
-    intro Hsucctm. specialize (Hbt Hsucctm). now inversion Hbt.
-Qed.
+    pose proof compile_tcompile wreg [] rer as Hcompile_tcompile.
+    pose proof tmatcher_bt rer lreg wreg Hcasesenst Hnomultiline HdotAll Hequiv wreg lreg [] as Hbt.
+    specialize_prove Hbt by constructor. specialize (Hbt Hequiv).
+
+    destruct Semantics.compileSubPattern as [m|] eqn:Heqm; simpl. 2: discriminate.
+    destruct tCompileSubPattern as [tm|] eqn:Heqtm; simpl. 2: discriminate.
+    specialize (Hcompile_tcompile m tm forward Heqm Heqtm str).
+    specialize (Hbt tm forward Heqtm).
+    intros Heqmatcher Heqtmatcher. injection Heqmatcher as <-. injection Heqtmatcher as <-.
+    intros Heqres Heqtres. subst res tres.
+    destruct negb. (* Negative length! *) 1: { split. - constructor. - discriminate. }
+    split.
+    - apply Hcompile_tcompile. + apply id_equiv. + reflexivity.
+    - specialize (Hbt id_tmcont [] str (id_tmcont_valid rer str forward)).
+      specialize (Hbt (init_input str) (MSInput.init_input_compat str)).
+      set (ms := match_state str 0 _). specialize (Hbt ms t).
+      specialize_prove Hbt by apply MSInput.init_ms_matches_inp. simpl in Hbt.
+      intro Hsucctm. specialize (Hbt Hsucctm). now inversion Hbt.
+  Qed.
+End LWEquivMain.
