warblreequiv/LWEquivTMatcher.v
@@ -18,410 +18,414 @@ Local Open Scope bool_scope.
    The equivalence itself is defined in LWEquivTMatcherDef.v. *)
 (* TODO Zero group *)
 
-(** ** The identity continuations. *)
-Definition id_mcont: MatcherContinuation := fun x => Success (Some x).
-Definition id_tmcont: TMatcherContinuation := fun _ => Success Match.
+Section LWEquivTMatcher.
+  Context `{characterClass: Character.class}.
 
-(* These two continuations are easily equivalent (under all input strings
-   and both directions and with no groups opened). *)
-Lemma id_equiv: forall str0 dir, equiv_tree_mcont str0 id_mcont id_tmcont nil dir.
-Proof.
-  constructor. reflexivity.
-Qed.
+  (** ** The identity continuations. *)
+  Definition id_mcont: MatcherContinuation := fun x => Success (Some x).
+  Definition id_tmcont: TMatcherContinuation := fun _ => Success Match.
 
-
-(** ** Lemma for repeated matching. *)
-Lemma repeatMatcher'_tRepeatMatcher':
-  (* For all pairs of a matcher m and a tree matcher tm *)
-  forall (str0: string) (m: Matcher) (tm: TMatcher) (dir: Direction) (greedy: bool)
-    (parenIndex parenCount: non_neg_integer),
-    (* that are equivalent, *)
-    equiv_tree_matcher str0 m tm dir ->
-    (* for any fuel, min and max, *)
-    forall fuel: nat,
-    forall (min: non_neg_integer) (max: non_neg_integer_or_inf),
-      (* the corresponding repeat matcher and tree matcher are equivalent with the same direction. *)
-      equiv_tree_matcher str0
-        (fun ms mc => Semantics.repeatMatcher' m min max greedy ms mc parenIndex parenCount fuel)
-        (fun ms tmc => tRepeatMatcher' tm dir min max greedy ms tmc parenIndex parenCount fuel) dir.
-Proof.
-  intros str0 m tm dir greedy parenIndex parenCount Hm_tm_equiv fuel.
-  induction fuel as [|fuel IHfuel].
-  1: constructor.
-  
-  intros min max mc tmc gl Hequivcont ms Hms_str0. simpl.
-  destruct (max =? 0)%NoI eqn:Hmax0; simpl.
-  (* Case max = 0: use hypothesis on continuation *)
-  1: { unfold equiv_tree_mcont in Hequivcont. now apply Hequivcont. }
-
-  (* Case max > 0 *)
-  destruct List.List.Update.Nat.Batch.update as [cap'|] eqn:Heqcap'; simpl. 2: constructor.
-  set (match_state (MatchState.input ms) (MatchState.endIndex ms) cap')
-    as ms_reset.
-  (* tmcnext and mcnext perform the progress check, then if this check succeeds, *)
-  (* perform the recursive call with decreased min/max. *)
-  set (fun y: MatchState => _) as tmcnext.
-  set (fun (y: MatchState) => (_: MatchResult)) as mcnext.
-  (* These two continuations are equivalent. *)
-  assert (equiv_tree_mcont str0 mcnext tmcnext gl dir) as Hequivnext. {
-    intros ms1 Hms1_str0.
-    unfold mcnext, tmcnext.
-    (* Case analysis on whether the progress check fails *)
-    destruct ((min ==? 0)%wt && _)%bool eqn:Hprogress; simpl.
-    - (* Fails *) constructor. reflexivity.
-    - (* Succeeds *)
-      set (if (min ==? 0)%wt then 0 else min - 1) as nextmin.
-      set (if (max =? +∞)%NoI then +∞ else (max - 1)%NoI) as nextmax.
-      specialize (IHfuel nextmin nextmax mc tmc gl Hequivcont ms1 Hms1_str0).
-      destruct (min ==? 0)%wt; inversion IHfuel; simpl; constructor; auto.
-  }
-  (* Therefore, the results of matching the inner regexp, then looping, are *)
-  (* equivalent. *)
-  assert (equiv_results (tm ms_reset tmcnext) ms_reset gl dir
-            (m ms_reset mcnext))
-    as Hequiv_loop. {
-    specialize (Hm_tm_equiv mcnext tmcnext gl Hequivnext ms_reset).
-    specialize_prove Hm_tm_equiv by now simpl.
-    inversion Hm_tm_equiv; now constructor.
-  }
-
-  assert ((reset_groups_ms (F := MatchError) (List.seq (parenIndex + 1) parenCount) ms) = ms_reset) as RESET_GROUPS by (eapply capture_reset_lw_same; eauto; reflexivity).
-  (* By hypothesis, the results of exiting the loop are equivalent. *)
-  pose proof Hequivcont ms Hms_str0 as Hequiv_exit.
-  assert (equiv_results
-            (let! z =<< tm ms_reset tmcnext in Success (GroupAction (Reset (List.seq (parenIndex + 1) parenCount)) z))
-            ms gl dir (m ms_reset mcnext)) as Hequiv_loopreset. {
-    inversion Hequiv_loop; simpl; constructor.
-    simpl. rewrite RESET_GROUPS. assumption.
-  }
-  destruct (negb (min =? 0)) eqn:Hmin_nonzero; simpl. 1: apply Hequiv_loopreset.
-  (* Case min = 0 *)
-  destruct greedy.
-  - setoid_rewrite func_monad_swap
-       with (f1 := fun z => GroupAction (Reset (List.seq (parenIndex + 1)
-                                                       parenCount)) z)
-            (f2 := id).
-     apply equiv_choice; try assumption.
-     rewrite monad_id. assumption.
-  - setoid_rewrite func_monad_swap
-       with (f2 := fun z => GroupAction (Reset (List.seq (parenIndex + 1)
-                                                       parenCount)) z)
-            (f1 := id).
-    apply equiv_choice; try assumption.
-    rewrite monad_id. assumption.
-Qed.
+  (* These two continuations are easily equivalent (under all input strings
+     and both directions and with no groups opened). *)
+  Lemma id_equiv: forall str0 dir, equiv_tree_mcont str0 id_mcont id_tmcont nil dir.
+  Proof.
+    constructor. reflexivity.
+  Qed.
 
 
-(** ** Lemma for character set matchers. *)
-Lemma charset_tcharset:
-  forall rer m tm charset str0 invert dir
-    (Heqm: Semantics.characterSetMatcher rer charset invert dir = m)
-    (Heqtm: tCharacterSetMatcher rer charset invert dir = tm),
-    equiv_tree_matcher str0 m tm dir.
-Proof.
-  intros. intros mc tmc gl Hequiv ms Hmsstr0.
-  subst m tm.
-  unfold tCharacterSetMatcher, Semantics.characterSetMatcher. simpl.
-  set (nextend := if (dir ==? forward)%wt then _ else _).
-  set ((_ <? 0)%Z || _)%bool as oob. destruct oob eqn:Hoob.
-  1: { constructor. reflexivity. }
-  
-  set (Z.min _ _) as index.
-  remember (List.List.Indexing.Int.indexing _ _) as readchr.
-  destruct readchr as [readchr|]; simpl. 2: constructor.
-  set (CharSet.exist_canonicalized _ _ _) as read_matches.
-  destruct ((if invert then false else true) && _); simpl. 1: constructor; reflexivity.
-  destruct ((if invert then true else false) && _); simpl. 1: constructor; reflexivity.
-  remember (match_state _ _ _) as ms'.
-  specialize (Hequiv ms').
-  specialize_prove Hequiv. { rewrite Heqms'; auto. }
-  destruct (tmc ms') as [child|]; simpl. 2: constructor.
-  destruct (mc ms') as [res|]; simpl. 2: constructor.
-  constructor.
-  (*replace index with (MatchState.endIndex ms) in Heqreadchr by lia.*)
-  inversion Hequiv as [child0 ms'0 gl0 dir0 res0 Hequiv' Heqchild0 Heqms'0 Heqgl0 Heqdir0 Heqres0 | |].
-  unfold nextend in Heqms'.
-  destruct dir; simpl in *; unfold advance_ms; rewrite <- Heqms'; rewrite <- Hequiv'; reflexivity.
-Qed.
+  (** ** Lemma for repeated matching. *)
+  Lemma repeatMatcher'_tRepeatMatcher':
+    (* For all pairs of a matcher m and a tree matcher tm *)
+    forall (str0: string) (m: Matcher) (tm: TMatcher) (dir: Direction) (greedy: bool)
+      (parenIndex parenCount: non_neg_integer),
+      (* that are equivalent, *)
+      equiv_tree_matcher str0 m tm dir ->
+      (* for any fuel, min and max, *)
+      forall fuel: nat,
+      forall (min: non_neg_integer) (max: non_neg_integer_or_inf),
+        (* the corresponding repeat matcher and tree matcher are equivalent with the same direction. *)
+        equiv_tree_matcher str0
+          (fun ms mc => Semantics.repeatMatcher' m min max greedy ms mc parenIndex parenCount fuel)
+          (fun ms tmc => tRepeatMatcher' tm dir min max greedy ms tmc parenIndex parenCount fuel) dir.
+  Proof.
+    intros str0 m tm dir greedy parenIndex parenCount Hm_tm_equiv fuel.
+    induction fuel as [|fuel IHfuel].
+    1: constructor.
 
+    intros min max mc tmc gl Hequivcont ms Hms_str0. simpl.
+    destruct (max =? 0)%NoI eqn:Hmax0; simpl.
+    (* Case max = 0: use hypothesis on continuation *)
+    1: { unfold equiv_tree_mcont in Hequivcont. now apply Hequivcont. }
 
-(** ** Lemma for lookarounds. *)
-
-(* A dummy match state to be able to discriminate; probably not strictly necessary. *)
-Definition dummy_match_state: MatchState := match_state nil 0%Z nil.
-
-(* The lemma; lkdir is the lookaround direction, pos is the lookaround positivity, lkreg is the lookaround regex. *)
-Lemma compile_tcompile_lk:
-  forall lkdir pos lkreg rer
-    (IH:
-      forall ctx m tm dir
-        (Heqm: Semantics.compileSubPattern lkreg ctx rer dir = Success m)
-        (Heqtm: tCompileSubPattern lkreg ctx rer dir = Success tm),
-        forall str0, equiv_tree_matcher str0 m tm dir),
-  forall ctx m tm dir
-    (Heqm: Semantics.compileSubPattern ((to_warblre_lookaround lkdir pos) lkreg) ctx rer dir = Success m)
-    (Heqtm: tLookaroundMatcher tCompileSubPattern lkdir pos lkreg ctx rer dir = Success tm),
-  forall str0, equiv_tree_matcher str0 m tm dir.
-Proof.
-  intros. pose proof (lookaroundMatcher_fact lkdir pos lkreg ctx rer dir) as Hfact. rewrite Heqm in Hfact. clear Heqm.
-  unfold tLookaroundMatcher in Heqtm. unfold lookaroundMatcher in Hfact.
-  destruct Semantics.compileSubPattern as [mlk|] eqn:Heqmlk; simpl in *. 2: discriminate (Hfact id_mcont dummy_match_state).
-  destruct tCompileSubPattern as [tmlk|] eqn:Heqtmlk; simpl in *. 2: discriminate.
-  injection Heqtm as <-. unfold equiv_tree_matcher.
-  intros mc tmc gl Hequivcont. unfold equiv_tree_mcont.
-  intros ms Hmsstr0. specialize (Hfact mc ms). injection Hfact as ->.
-  specialize (IH _ mlk tmlk lkdir Heqmlk Heqtmlk str0 id_mcont id_tmcont nil (id_equiv str0 lkdir) ms Hmsstr0). simpl in *.
-  destruct tmlk as [tlk|] eqn:Htlk; try solve[constructor]. simpl.
-  destruct mlk as [mslkopt|] eqn:Hmslkopt; try solve[constructor]. simpl.
-  inversion IH as [tlk' ms' nil' lkdir' mslkopt' IH' | |]. subst tlk' ms' nil' lkdir' mslkopt'.
-  rewrite <- IH'. unfold equiv_tree_mcont in Hequivcont.
-  destruct pos; destruct mslkopt as [mslk|]; simpl; try solve[now constructor].
-  - set (msafterlk := match_state _ _ _). specialize (Hequivcont msafterlk Hmsstr0).
-    inversion Hequivcont as [t1 msafterlk' gl' r Hcontequiv' | |]. 2,3: constructor.
-    constructor. simpl. replace (Regex.positivity _) with true by now destruct lkdir. replace (Regex.lk_dir _) with lkdir by now destruct lkdir. rewrite <- IH'. auto.
-  - specialize (Hequivcont ms Hmsstr0). inversion Hequivcont as [t1 msafterlk' gl' r Hcontequiv' | |]. 2,3: constructor.
-    simpl. constructor. simpl. replace (Regex.positivity _) with false by now destruct lkdir. replace (Regex.lk_dir _) with lkdir by now destruct lkdir. rewrite <- IH'. auto.
-Qed.
-
-
-(** ** Lemma for AtomEscs *)
-Lemma compile_tcompile_atomescape:
-  forall ae ctx rer m tm dir
-    (Heqm: Semantics.compileSubPattern (AtomEsc ae) ctx rer dir = Success m)
-    (Heqtm: tCompileSubPattern (AtomEsc ae) ctx rer dir = Success tm),
-  forall str0, equiv_tree_matcher str0 m tm dir.
-Proof.
-  intros ae ctx rer m tm dir. simpl. destruct ae; try discriminate.
-  - (* ACharacterClassEsc *)
-    destruct esc.
-    (* \d, \D, \s, \S, \w, \W *)
-    1-6: intros; injection Heqm as <-; injection Heqtm as <-; eapply charset_tcharset; reflexivity.
-    + (* Unicode property *)
-      destruct p.
-    + (* Negative unicode property *)
-      destruct p.
-  - (* ACharacterEsc *)
-    destruct esc; simpl.
-    + (* ControlEsc *)
-      destruct esc; intros; injection Heqm as <-; injection Heqtm as <-; eapply charset_tcharset; reflexivity.
-    + (* AsciiControlEsc *)
-      intros; injection Heqm as <-; injection Heqtm as <-; eapply charset_tcharset; reflexivity.
-    + (* esc_Zero *)
-      intros; injection Heqm as <-; injection Heqtm as <-; eapply charset_tcharset; reflexivity.
-    + (* HexEscape *)
-      intros; injection Heqm as <-; injection Heqtm as <-; eapply charset_tcharset; reflexivity.
-    + (* UnicodeEsc *)
-      destruct seq; intros; injection Heqm as <-; injection Heqtm as <-; eapply charset_tcharset; reflexivity.
-    + (* IdentityEsc *)
-      intros; injection Heqm as <-; injection Heqtm as <-; eapply charset_tcharset; reflexivity.
-Qed.
-
-(** ** Main theorem *)
-Theorem compile_tcompile:
-  forall reg ctx rer m tm dir (* for all regexes, contexts, RegExpRecords and directions, *)
-    (* if the compilations of the regexes into a matcher and a tree matcher succeed, *)
-    (Heqm: Semantics.compileSubPattern reg ctx rer dir = Success m)
-    (Heqtm: tCompileSubPattern reg ctx rer dir = Success tm),
-    (* then the resulting matcher and tree matcher are equivalent. *)
-  forall str0, equiv_tree_matcher str0 m tm dir.
-Proof.
-  intros reg ctx rer.
-  revert ctx.
-  induction reg as [
-    |
-    chr |
-    |
-    ae |
-    cc |
-    wr1 IH1 wr2 IH2 |
-    wr IH q |
-    wr1 IH1 wr2 IH2 |
-    name wr IH |
-    |
-    |
-    |
-    |
-    wr IH |
-    wr IH |
-    wr IH |
-    wr IH
-  ]; try discriminate.
-
-  - (* Empty *)
-    intros. injection Heqm as <-. injection Heqtm as <-.
-    intros mc tmc gl Hequiv ms Hmsstr0.
-    now apply Hequiv.
-
-  - (* Character *)
-    intros. injection Heqm as <-. injection Heqtm as <-. eapply charset_tcharset; reflexivity.
-    
-  - (* Dot; same as character *)
-    intros. injection Heqm as <-. injection Heqtm as <-. eapply charset_tcharset; reflexivity.
-
-  - (* AtomEsc *)
-    intros. eapply compile_tcompile_atomescape; eauto.
-
-  - (* CharacterClass *)
-    simpl. intros. destruct Semantics.compileCharacterClass; simpl in *. 2: discriminate. injection Heqm as <-. injection Heqtm as <-. eapply charset_tcharset; reflexivity.
-
-  - (* Disjunction *)
-    simpl. intros.
-    remember (Disjunction_left wr2 :: ctx)%list as ctxleft.
-    remember (Disjunction_right wr1 :: ctx)%list as ctxright.
-    specialize (IH1 ctxleft).
-    specialize (IH2 ctxright).
-    destruct (Semantics.compileSubPattern wr1 _ _ _) as [m1|] eqn:Heqm1; simpl. 2: discriminate.
-    destruct (Semantics.compileSubPattern wr2 _ _ _) as [m2|] eqn:Heqm2; simpl. 2: discriminate.
-    destruct (tCompileSubPattern wr1 _ _ _) as [tm1|] eqn:Heqtm1; simpl. 2: discriminate.
-    destruct (tCompileSubPattern wr2 _ _ _) as [tm2|] eqn:Heqtm2; simpl. 2: discriminate.
-    simpl in *.
-    intros mc tmc gl Hequiv ms' Hms'str0.
-    specialize (IH1 m1 tm1 dir Heqm1 Heqtm1 str0 mc tmc gl Hequiv ms' Hms'str0).
-    specialize (IH2 m2 tm2 dir Heqm2 Heqtm2 str0 mc tmc gl Hequiv ms' Hms'str0).
-    simpl in *.
-    injection Heqtm as <-.
-    destruct (tm1 ms' tmc) as [t1|] eqn:Heqt1; simpl. 2: constructor.
-    destruct (tm2 ms' tmc) as [t2|] eqn:Heqt2; simpl. 2: constructor.
-    injection Heqm as <-.
-    destruct (m1 ms' mc) as [r|] eqn:Heqr; simpl. 2: constructor.
-    destruct r eqn:?; simpl.
-    + constructor. inversion IH1 as [t1' ms'' gl' dir' res IH1' Heqt1' Heqms'' Heqgl' Heqdir' Heqres | |].
-      simpl. rewrite <- IH1'. reflexivity.
-    + destruct (m2 ms' mc) as [r2|] eqn:Heqr2; simpl. 2: constructor.
-      constructor.
-      inversion IH1 as [t1' ms'' gl' dir' res IH1' Heqt1' Heqms'' Heqgl' Heqdir' Heqres | |].
-      clear t1' ms'' gl' dir' res Heqt1' Heqms'' Heqgl' Heqdir' Heqres.
-      simpl. rewrite <- IH1'. simpl.
-      now inversion IH2.
-
-  - (* Quantifier *)
-    simpl. intros.
-    remember (Quantified_inner q :: ctx)%list as ctx'.
-    specialize (IH ctx').
-    destruct Semantics.compileSubPattern as [msub|] eqn:Heqmsub; simpl. 2: discriminate.
-    destruct tCompileSubPattern as [tmsub|] eqn:Heqtmsub; simpl. 2: discriminate.
-    specialize (IH msub tmsub dir Heqmsub Heqtmsub).
-    simpl in *.
-    destruct negb; simpl. 1: discriminate.
-    unfold equiv_tree_matcher. intros mc tmc gl Hequivcont.
-    unfold equiv_tree_mcont. intro ms.
-    unfold Semantics.repeatMatcher in Heqm. unfold tRepeatMatcher in Heqtm.
-    injection Heqm as <-. injection Heqtm as <-.
-    now apply repeatMatcher'_tRepeatMatcher'.
-
-  - (* Sequence *)
-    simpl. intros.
-    remember (Seq_left wr2 :: ctx)%list as ctxleft.
-    remember (Seq_right wr1 :: ctx)%list as ctxright.
-    specialize (IH1 ctxleft). specialize (IH2 ctxright).
-    destruct (Semantics.compileSubPattern wr1 _ _ _) as [m1|] eqn:Heqm1; simpl. 2: discriminate.
-    destruct (Semantics.compileSubPattern wr2 _ _ _) as [m2|] eqn:Heqm2; simpl. 2: discriminate.
-    destruct (tCompileSubPattern wr1 _ _ _) as [tm1|] eqn:Heqtm1; simpl. 2: discriminate.
-    destruct (tCompileSubPattern wr2 _ _ _) as [tm2|] eqn:Heqtm2; simpl. 2: discriminate.
-    simpl in *. destruct dir; injection Heqm as <-; injection Heqtm as <-; intros mc tmc gl Hequiv ms.
-    + specialize (IH2 m2 tm2 forward Heqm2 Heqtm2 str0 mc tmc gl Hequiv).
-      specialize (IH1 m1 tm1 forward Heqm1 Heqtm1 str0 (fun ms0 => m2 ms0 mc) (fun ms0 => tm2 ms0 tmc) gl IH2 ms). auto.
-    + specialize (IH1 m1 tm1 backward Heqm1 Heqtm1 str0 mc tmc gl Hequiv).
-      specialize (IH2 m2 tm2 backward Heqm2 Heqtm2 str0 (fun ms0 => m1 ms0 mc) (fun ms0 => tm1 ms0 tmc) gl IH1 ms). auto.
-
-  - (* Group *)
-    simpl. intros.
-    remember (Group_inner name :: ctx)%list as ctx'. specialize (IH ctx').
-    destruct (Semantics.compileSubPattern wr ctx' rer dir) as [msub|] eqn:Heqmsub; simpl. 2: discriminate.
-    destruct (tCompileSubPattern wr ctx' rer dir) as [tmsub|] eqn:Heqtmsub; simpl. 2: discriminate.
-    intros mc tmc gl Hequiv ms Hmsstr0.
-    simpl in *.
-    injection Heqm as <-. injection Heqtm as <-.
-    remember (fun y : MatchState => _) as treecont.
-    remember (fun y : MatchState => let! r =<< _ in let! cap =<< _ in mc _) as origcont.
-    remember (StaticSemantics.countLeftCapturingParensBefore _ ctx + 1) as gid.
-    set (gl' := ((gid, MatchState.endIndex ms, dir)::gl)%list).
-    specialize (IH msub tmsub dir Heqmsub Heqtmsub str0 origcont treecont gl').
-    specialize_prove IH. {
-      intros y Hy_ms_sameinp.
-      rewrite Heqtreecont, Heqorigcont.
-      set (extr1 := MatchState.endIndex ms). set (extr2 := MatchState.endIndex y).
-      remember (if (dir ==? forward)%wt then _ else _) as rangeresult. destruct rangeresult as [r|] eqn:Heqrange; simpl. 2: constructor.
-      destruct (gid =? 0) eqn:Hgid_nonzero; simpl. 1: constructor.
-      destruct List.List.Update.Nat.One.update as [cap'|] eqn:Hcapupd; simpl. 2: constructor.
-      remember (match_state _ _ cap') as ms'.
-      destruct (tmc ms') as [t|] eqn:Heqt; simpl. 2: constructor.
-      destruct (mc ms') as [res|] eqn:Heqres; simpl. 2: constructor.
-      constructor. simpl. rewrite EqDec.reflb. rewrite Hgid_nonzero.
-      replace (Some (capture_range _ _)) with r.
-      2: {
-        destruct dir; simpl in *; destruct negb; try solve[discriminate]; inversion Heqrangeresult; auto.
-      }
-      unfold CaptureRange_or_undefined in Hcapupd. rewrite Hcapupd.
-      specialize (Hequiv ms').
-      specialize_prove Hequiv. { rewrite Heqms'; auto. }
-      rewrite Heqt, Heqres in Hequiv.
-      inversion Hequiv as [t' ms'' gl'' dir' res' Hequiv' Heqt' Heqms'' Heqgl'' Heqdir' Heqres' | |].
-      clear t' ms'' gl'' res' Heqt' Heqms'' Heqgl'' Heqres'.
-      rewrite Heqms' in Hequiv'. rewrite Hy_ms_sameinp. rewrite Hmsstr0 in Hequiv'.
-      assumption.
+    (* Case max > 0 *)
+    destruct List.List.Update.Nat.Batch.update as [cap'|] eqn:Heqcap'; simpl. 2: constructor.
+    set (match_state (MatchState.input ms) (MatchState.endIndex ms) cap')
+      as ms_reset.
+    (* tmcnext and mcnext perform the progress check, then if this check succeeds, *)
+    (* perform the recursive call with decreased min/max. *)
+    set (fun y: MatchState => _) as tmcnext.
+    set (fun (y: MatchState) => (_: MatchResult)) as mcnext.
+    (* These two continuations are equivalent. *)
+    assert (equiv_tree_mcont str0 mcnext tmcnext gl dir) as Hequivnext. {
+      intros ms1 Hms1_str0.
+      unfold mcnext, tmcnext.
+      (* Case analysis on whether the progress check fails *)
+      destruct ((min ==? 0)%wt && _)%bool eqn:Hprogress; simpl.
+      - (* Fails *) constructor. reflexivity.
+      - (* Succeeds *)
+        set (if (min ==? 0)%wt then 0 else min - 1) as nextmin.
+        set (if (max =? +∞)%NoI then +∞ else (max - 1)%NoI) as nextmax.
+        specialize (IHfuel nextmin nextmax mc tmc gl Hequivcont ms1 Hms1_str0).
+        destruct (min ==? 0)%wt; inversion IHfuel; simpl; constructor; auto.
     }
-    specialize (IH ms Hmsstr0). simpl in *.
-    destruct (tmsub ms treecont) as [t|] eqn:Heqt; simpl. 2: constructor.
-    destruct (msub ms origcont) as [res|] eqn:Heqres; simpl. 2: constructor.
-    constructor. inversion IH. auto.
+    (* Therefore, the results of matching the inner regexp, then looping, are *)
+    (* equivalent. *)
+    assert (equiv_results (tm ms_reset tmcnext) ms_reset gl dir
+              (m ms_reset mcnext))
+      as Hequiv_loop. {
+      specialize (Hm_tm_equiv mcnext tmcnext gl Hequivnext ms_reset).
+      specialize_prove Hm_tm_equiv by now simpl.
+      inversion Hm_tm_equiv; now constructor.
+    }
 
-  - (* Input start *)
-    simpl. intros _ m tm dir Heqm Heqtm. injection Heqm as <-. injection Heqtm as <-.
-    intro str0. unfold equiv_tree_matcher. intros mc tmc gl Hequivcont.
-    unfold equiv_tree_mcont. intros ms Hmsstr0.
-    destruct (if (_: bool) then Success true else _) as [anchormatch|]; simpl. 2: constructor.
-    destruct anchormatch.
-    + unfold equiv_tree_mcont in Hequivcont. specialize (Hequivcont ms Hmsstr0). inversion Hequivcont; try solve[constructor]; simpl.
-      constructor. auto.
-    + constructor. auto.
+    assert ((reset_groups_ms (F := MatchError) (List.seq (parenIndex + 1) parenCount) ms) = ms_reset) as RESET_GROUPS by (eapply capture_reset_lw_same; eauto; reflexivity).
+    (* By hypothesis, the results of exiting the loop are equivalent. *)
+    pose proof Hequivcont ms Hms_str0 as Hequiv_exit.
+    assert (equiv_results
+              (let! z =<< tm ms_reset tmcnext in Success (GroupAction (Reset (List.seq (parenIndex + 1) parenCount)) z))
+              ms gl dir (m ms_reset mcnext)) as Hequiv_loopreset. {
+      inversion Hequiv_loop; simpl; constructor.
+      simpl. rewrite RESET_GROUPS. assumption.
+    }
+    destruct (negb (min =? 0)) eqn:Hmin_nonzero; simpl. 1: apply Hequiv_loopreset.
+    (* Case min = 0 *)
+    destruct greedy.
+    - setoid_rewrite func_monad_swap
+         with (f1 := fun z => GroupAction (Reset (List.seq (parenIndex + 1)
+                                                         parenCount)) z)
+              (f2 := id).
+       apply equiv_choice; try assumption.
+       rewrite monad_id. assumption.
+    - setoid_rewrite func_monad_swap
+         with (f2 := fun z => GroupAction (Reset (List.seq (parenIndex + 1)
+                                                         parenCount)) z)
+              (f1 := id).
+      apply equiv_choice; try assumption.
+      rewrite monad_id. assumption.
+  Qed.
 
-  - (* Input end: same as input start, but the placeholders in the first destruct are different *)
-    simpl. intros _ m tm dir Heqm Heqtm. injection Heqm as <-. injection Heqtm as <-.
-    intros str0 mc tmc gl Hequivcont ms Hmsstr0.
-    destruct (if (_: bool) then Success true else _) as [anchormatch|]; simpl. 2: constructor.
-    destruct anchormatch.
-    + unfold equiv_tree_mcont in Hequivcont. specialize (Hequivcont ms Hmsstr0). inversion Hequivcont; try solve[constructor]; simpl.
-      constructor. auto.
-    + constructor. auto.
 
-  (* Word boundary *)
-  - simpl. intros _ m tm dir Hcompsucc Htcompsucc str0. injection Hcompsucc as <-. injection Htcompsucc as <-.
-    unfold equiv_tree_matcher.
+  (** ** Lemma for character set matchers. *)
+  Lemma charset_tcharset:
+    forall rer m tm charset str0 invert dir
+      (Heqm: Semantics.characterSetMatcher rer charset invert dir = m)
+      (Heqtm: tCharacterSetMatcher rer charset invert dir = tm),
+      equiv_tree_matcher str0 m tm dir.
+  Proof.
+    intros. intros mc tmc gl Hequiv ms Hmsstr0.
+    subst m tm.
+    unfold tCharacterSetMatcher, Semantics.characterSetMatcher. simpl.
+    set (nextend := if (dir ==? forward)%wt then _ else _).
+    set ((_ <? 0)%Z || _)%bool as oob. destruct oob eqn:Hoob.
+    1: { constructor. reflexivity. }
+
+    set (Z.min _ _) as index.
+    remember (List.List.Indexing.Int.indexing _ _) as readchr.
+    destruct readchr as [readchr|]; simpl. 2: constructor.
+    set (CharSet.exist_canonicalized _ _ _) as read_matches.
+    destruct ((if invert then false else true) && _); simpl. 1: constructor; reflexivity.
+    destruct ((if invert then true else false) && _); simpl. 1: constructor; reflexivity.
+    remember (match_state _ _ _) as ms'.
+    specialize (Hequiv ms').
+    specialize_prove Hequiv. { rewrite Heqms'; auto. }
+    destruct (tmc ms') as [child|]; simpl. 2: constructor.
+    destruct (mc ms') as [res|]; simpl. 2: constructor.
+    constructor.
+    (*replace index with (MatchState.endIndex ms) in Heqreadchr by lia.*)
+    inversion Hequiv as [child0 ms'0 gl0 dir0 res0 Hequiv' Heqchild0 Heqms'0 Heqgl0 Heqdir0 Heqres0 | |].
+    unfold nextend in Heqms'.
+    destruct dir; simpl in *; unfold advance_ms; rewrite <- Heqms'; rewrite <- Hequiv'; reflexivity.
+  Qed.
+
+
+  (** ** Lemma for lookarounds. *)
+
+  (* A dummy match state to be able to discriminate; probably not strictly necessary. *)
+  Definition dummy_match_state: MatchState := match_state nil 0%Z nil.
+
+  (* The lemma; lkdir is the lookaround direction, pos is the lookaround positivity, lkreg is the lookaround regex. *)
+  Lemma compile_tcompile_lk:
+    forall lkdir pos lkreg rer
+      (IH:
+        forall ctx m tm dir
+          (Heqm: Semantics.compileSubPattern lkreg ctx rer dir = Success m)
+          (Heqtm: tCompileSubPattern lkreg ctx rer dir = Success tm),
+          forall str0, equiv_tree_matcher str0 m tm dir),
+    forall ctx m tm dir
+      (Heqm: Semantics.compileSubPattern ((to_warblre_lookaround lkdir pos) lkreg) ctx rer dir = Success m)
+      (Heqtm: tLookaroundMatcher tCompileSubPattern lkdir pos lkreg ctx rer dir = Success tm),
+    forall str0, equiv_tree_matcher str0 m tm dir.
+  Proof.
+    intros. pose proof (lookaroundMatcher_fact lkdir pos lkreg ctx rer dir) as Hfact. setoid_rewrite Heqm in Hfact. clear Heqm.
+    unfold tLookaroundMatcher in Heqtm. unfold lookaroundMatcher in Hfact.
+    destruct Semantics.compileSubPattern as [mlk|] eqn:Heqmlk; simpl in *. 2: discriminate (Hfact id_mcont dummy_match_state).
+    destruct tCompileSubPattern as [tmlk|] eqn:Heqtmlk; simpl in *. 2: discriminate.
+    injection Heqtm as <-. unfold equiv_tree_matcher.
     intros mc tmc gl Hequivcont. unfold equiv_tree_mcont.
-    intros ms Hmsstr0.
-    destruct Semantics.isWordChar as [a|] eqn:Hwca; simpl. 2: constructor.
-    destruct (Semantics.isWordChar rer (_ ms) (MatchState.endIndex ms)) as [b|] eqn:Hwcb; simpl. 2: constructor.
-    destruct (_ && _ || _ && _); simpl.
-    + unfold equiv_tree_mcont in Hequivcont. specialize (Hequivcont ms Hmsstr0).
-      destruct tmc as [t|]; simpl. 2: constructor.
-      destruct mc as [res|]; simpl. 2: constructor.
-      constructor. simpl. now inversion Hequivcont.
-    + constructor. reflexivity.
+    intros ms Hmsstr0. specialize (Hfact mc ms). injection Hfact as ->.
+    specialize (IH _ mlk tmlk lkdir Heqmlk Heqtmlk str0 id_mcont id_tmcont nil (id_equiv str0 lkdir) ms Hmsstr0). simpl in *.
+    destruct tmlk as [tlk|] eqn:Htlk; try solve[constructor]. simpl.
+    destruct mlk as [mslkopt|] eqn:Hmslkopt; try solve[constructor]. simpl.
+    inversion IH as [tlk' ms' nil' lkdir' mslkopt' IH' | |]. subst tlk' ms' nil' lkdir' mslkopt'.
+    rewrite <- IH'. unfold equiv_tree_mcont in Hequivcont.
+    destruct pos; destruct mslkopt as [mslk|]; simpl; try solve[now constructor].
+    - set (msafterlk := match_state _ _ _). specialize (Hequivcont msafterlk Hmsstr0).
+      inversion Hequivcont as [t1 msafterlk' gl' r Hcontequiv' | |]. 2,3: constructor.
+      constructor. simpl. replace (Regex.positivity _) with true by now destruct lkdir. replace (Regex.lk_dir _) with lkdir by now destruct lkdir. rewrite <- IH'. auto.
+    - specialize (Hequivcont ms Hmsstr0). inversion Hequivcont as [t1 msafterlk' gl' r Hcontequiv' | |]. 2,3: constructor.
+      simpl. constructor. simpl. replace (Regex.positivity _) with false by now destruct lkdir. replace (Regex.lk_dir _) with lkdir by now destruct lkdir. rewrite <- IH'. auto.
+  Qed.
 
-  (* Non word boundary; same proof as above, except the placeholders at the main destruct differ *)
-  - simpl. intros _ m tm dir Hcompsucc Htcompsucc str0. injection Hcompsucc as <-. injection Htcompsucc as <-.
-    unfold equiv_tree_matcher.
-    intros mc tmc gl Hequivcont. unfold equiv_tree_mcont.
-    intros ms Hmsstr0.
-    destruct Semantics.isWordChar as [a|] eqn:Hwca; simpl. 2: constructor.
-    destruct (Semantics.isWordChar rer (_ ms) (MatchState.endIndex ms)) as [b|] eqn:Hwcb; simpl. 2: constructor.
-    destruct (_ && _ || _ && _); simpl.
-    + unfold equiv_tree_mcont in Hequivcont. specialize (Hequivcont ms Hmsstr0).
-      destruct tmc as [t|]; simpl. 2: constructor.
-      destruct mc as [res|]; simpl. 2: constructor.
-      constructor. simpl. now inversion Hequivcont.
-    + constructor. reflexivity.
 
-    (* Positive lookahead *)
-  - simpl. intros. apply compile_tcompile_lk with (lkdir := forward) (pos := true) (lkreg := wr) (rer := rer) (ctx := ctx); auto.
+  (** ** Lemma for AtomEscs *)
+  Lemma compile_tcompile_atomescape:
+    forall ae ctx rer m tm dir
+      (Heqm: Semantics.compileSubPattern (AtomEsc ae) ctx rer dir = Success m)
+      (Heqtm: tCompileSubPattern (AtomEsc ae) ctx rer dir = Success tm),
+    forall str0, equiv_tree_matcher str0 m tm dir.
+  Proof.
+    intros ae ctx rer m tm dir. simpl. destruct ae; try discriminate.
+    - (* ACharacterClassEsc *)
+      destruct esc.
+      (* \d, \D, \s, \S, \w, \W *)
+      1-6: intros; injection Heqm as <-; injection Heqtm as <-; eapply charset_tcharset; reflexivity.
+      + (* Unicode property *)
+        destruct p.
+      + (* Negative unicode property *)
+        destruct p.
+    - (* ACharacterEsc *)
+      destruct esc; simpl.
+      + (* ControlEsc *)
+        destruct esc; intros; injection Heqm as <-; injection Heqtm as <-; eapply charset_tcharset; reflexivity.
+      + (* AsciiControlEsc *)
+        intros; injection Heqm as <-; injection Heqtm as <-; eapply charset_tcharset; reflexivity.
+      + (* esc_Zero *)
+        intros; injection Heqm as <-; injection Heqtm as <-; eapply charset_tcharset; reflexivity.
+      + (* HexEscape *)
+        intros; injection Heqm as <-; injection Heqtm as <-; eapply charset_tcharset; reflexivity.
+      + (* UnicodeEsc *)
+        destruct seq; intros; injection Heqm as <-; injection Heqtm as <-; eapply charset_tcharset; reflexivity.
+      + (* IdentityEsc *)
+        intros; injection Heqm as <-; injection Heqtm as <-; eapply charset_tcharset; reflexivity.
+  Qed.
 
-    (* Negative lookahead *)
-  - simpl. intros. apply compile_tcompile_lk with (lkdir := forward) (pos := false) (lkreg := wr) (rer := rer) (ctx := ctx); auto.
+  (** ** Main theorem *)
+  Theorem compile_tcompile:
+    forall reg ctx rer m tm dir (* for all regexes, contexts, RegExpRecords and directions, *)
+      (* if the compilations of the regexes into a matcher and a tree matcher succeed, *)
+      (Heqm: Semantics.compileSubPattern reg ctx rer dir = Success m)
+      (Heqtm: tCompileSubPattern reg ctx rer dir = Success tm),
+      (* then the resulting matcher and tree matcher are equivalent. *)
+    forall str0, equiv_tree_matcher str0 m tm dir.
+  Proof.
+    intros reg ctx rer.
+    revert ctx.
+    induction reg as [
+      |
+      chr |
+      |
+      ae |
+      cc |
+      wr1 IH1 wr2 IH2 |
+      wr IH q |
+      wr1 IH1 wr2 IH2 |
+      name wr IH |
+      |
+      |
+      |
+      |
+      wr IH |
+      wr IH |
+      wr IH |
+      wr IH
+    ]; try discriminate.
 
-    (* Positive lookbehind *)
-  - simpl. intros. apply compile_tcompile_lk with (lkdir := backward) (pos := true) (lkreg := wr) (rer := rer) (ctx := ctx); auto.
+    - (* Empty *)
+      intros. injection Heqm as <-. injection Heqtm as <-.
+      intros mc tmc gl Hequiv ms Hmsstr0.
+      now apply Hequiv.
 
-    (* Negative lookbehind *)
-  - simpl. intros. apply compile_tcompile_lk with (lkdir := backward) (pos := false) (lkreg := wr) (rer := rer) (ctx := ctx); auto.
-Qed.
+    - (* Character *)
+      intros. injection Heqm as <-. injection Heqtm as <-. eapply charset_tcharset; reflexivity.
+
+    - (* Dot; same as character *)
+      intros. injection Heqm as <-. injection Heqtm as <-. eapply charset_tcharset; reflexivity.
+
+    - (* AtomEsc *)
+      intros. eapply compile_tcompile_atomescape; eauto.
+
+    - (* CharacterClass *)
+      simpl. intros. destruct Semantics.compileCharacterClass; simpl in *. 2: discriminate. injection Heqm as <-. injection Heqtm as <-. eapply charset_tcharset; reflexivity.
+
+    - (* Disjunction *)
+      simpl. intros.
+      remember (Disjunction_left wr2 :: ctx)%list as ctxleft.
+      remember (Disjunction_right wr1 :: ctx)%list as ctxright.
+      specialize (IH1 ctxleft).
+      specialize (IH2 ctxright).
+      destruct (Semantics.compileSubPattern wr1 _ _ _) as [m1|] eqn:Heqm1; simpl. 2: discriminate.
+      destruct (Semantics.compileSubPattern wr2 _ _ _) as [m2|] eqn:Heqm2; simpl. 2: discriminate.
+      destruct tCompileSubPattern as [tm1|] eqn:Heqtm1 in Heqtm; simpl. 2: discriminate.
+      destruct tCompileSubPattern as [tm2|] eqn:Heqtm2 in Heqtm; simpl. 2: discriminate.
+      simpl in *.
+      intros mc tmc gl Hequiv ms' Hms'str0.
+      specialize (IH1 m1 tm1 dir Heqm1 Heqtm1 str0 mc tmc gl Hequiv ms' Hms'str0).
+      specialize (IH2 m2 tm2 dir Heqm2 Heqtm2 str0 mc tmc gl Hequiv ms' Hms'str0).
+      simpl in *.
+      injection Heqtm as <-.
+      destruct (tm1 ms' tmc) as [t1|] eqn:Heqt1; simpl. 2: constructor.
+      destruct (tm2 ms' tmc) as [t2|] eqn:Heqt2; simpl. 2: constructor.
+      injection Heqm as <-.
+      destruct (m1 ms' mc) as [r|] eqn:Heqr; simpl. 2: constructor.
+      destruct r eqn:?; simpl.
+      + constructor. inversion IH1 as [t1' ms'' gl' dir' res IH1' Heqt1' Heqms'' Heqgl' Heqdir' Heqres | |].
+        simpl. rewrite <- IH1'. reflexivity.
+      + destruct (m2 ms' mc) as [r2|] eqn:Heqr2; simpl. 2: constructor.
+        constructor.
+        inversion IH1 as [t1' ms'' gl' dir' res IH1' Heqt1' Heqms'' Heqgl' Heqdir' Heqres | |].
+        clear t1' ms'' gl' dir' res Heqt1' Heqms'' Heqgl' Heqdir' Heqres.
+        simpl. rewrite <- IH1'. simpl.
+        now inversion IH2.
+
+    - (* Quantifier *)
+      simpl. intros.
+      remember (Quantified_inner q :: ctx)%list as ctx'.
+      specialize (IH ctx').
+      destruct Semantics.compileSubPattern as [msub|] eqn:Heqmsub; simpl. 2: discriminate.
+      destruct tCompileSubPattern as [tmsub|] eqn:Heqtmsub; simpl. 2: discriminate.
+      specialize (IH msub tmsub dir Heqmsub Heqtmsub).
+      simpl in *.
+      destruct negb; simpl. 1: discriminate.
+      unfold equiv_tree_matcher. intros mc tmc gl Hequivcont.
+      unfold equiv_tree_mcont. intro ms.
+      unfold Semantics.repeatMatcher in Heqm. unfold tRepeatMatcher in Heqtm.
+      injection Heqm as <-. injection Heqtm as <-.
+      now apply repeatMatcher'_tRepeatMatcher'.
+
+    - (* Sequence *)
+      simpl. intros.
+      remember (Seq_left wr2 :: ctx)%list as ctxleft.
+      remember (Seq_right wr1 :: ctx)%list as ctxright.
+      specialize (IH1 ctxleft). specialize (IH2 ctxright).
+      destruct (Semantics.compileSubPattern wr1 _ _ _) as [m1|] eqn:Heqm1; simpl. 2: discriminate.
+      destruct (Semantics.compileSubPattern wr2 _ _ _) as [m2|] eqn:Heqm2; simpl. 2: discriminate.
+      destruct tCompileSubPattern as [tm1|] eqn:Heqtm1 in Heqtm; simpl. 2: discriminate.
+      destruct tCompileSubPattern as [tm2|] eqn:Heqtm2 in Heqtm; simpl. 2: discriminate.
+      simpl in *. destruct dir; injection Heqm as <-; injection Heqtm as <-; intros mc tmc gl Hequiv ms.
+      + specialize (IH2 m2 tm2 forward Heqm2 Heqtm2 str0 mc tmc gl Hequiv).
+        specialize (IH1 m1 tm1 forward Heqm1 Heqtm1 str0 (fun ms0 => m2 ms0 mc) (fun ms0 => tm2 ms0 tmc) gl IH2 ms). auto.
+      + specialize (IH1 m1 tm1 backward Heqm1 Heqtm1 str0 mc tmc gl Hequiv).
+        specialize (IH2 m2 tm2 backward Heqm2 Heqtm2 str0 (fun ms0 => m1 ms0 mc) (fun ms0 => tm1 ms0 tmc) gl IH1 ms). auto.
+
+    - (* Group *)
+      simpl. intros.
+      remember (Group_inner name :: ctx)%list as ctx'. specialize (IH ctx').
+      destruct (Semantics.compileSubPattern wr ctx' rer dir) as [msub|] eqn:Heqmsub; simpl. 2: discriminate.
+      destruct tCompileSubPattern as [tmsub|] eqn:Heqtmsub in Heqtm; simpl. 2: discriminate.
+      intros mc tmc gl Hequiv ms Hmsstr0.
+      simpl in *.
+      injection Heqm as <-. injection Heqtm as <-.
+      remember (fun y : MatchState => _) as treecont.
+      remember (fun y : MatchState => let! r =<< _ in let! cap =<< _ in mc _) as origcont.
+      remember (StaticSemantics.countLeftCapturingParensBefore _ ctx + 1) as gid.
+      set (gl' := ((gid, MatchState.endIndex ms, dir)::gl)%list).
+      specialize (IH msub tmsub dir Heqmsub Heqtmsub str0 origcont treecont gl').
+      specialize_prove IH. {
+        intros y Hy_ms_sameinp.
+        rewrite Heqtreecont, Heqorigcont.
+        set (extr1 := MatchState.endIndex ms). set (extr2 := MatchState.endIndex y).
+        remember (if (dir ==? forward)%wt then _ else _) as rangeresult. destruct rangeresult as [r|] eqn:Heqrange; simpl. 2: constructor.
+        destruct (gid =? 0) eqn:Hgid_nonzero; simpl. 1: constructor.
+        destruct List.List.Update.Nat.One.update as [cap'|] eqn:Hcapupd; simpl. 2: constructor.
+        remember (match_state _ _ cap') as ms'.
+        destruct (tmc ms') as [t|] eqn:Heqt; simpl. 2: constructor.
+        destruct (mc ms') as [res|] eqn:Heqres; simpl. 2: constructor.
+        constructor. simpl. rewrite EqDec.reflb. rewrite Hgid_nonzero.
+        replace (Some (capture_range _ _)) with r.
+        2: {
+          destruct dir; simpl in *; destruct negb; try solve[discriminate]; inversion Heqrangeresult; auto.
+        }
+        unfold CaptureRange_or_undefined in Hcapupd. rewrite Hcapupd.
+        specialize (Hequiv ms').
+        specialize_prove Hequiv. { rewrite Heqms'; auto. }
+        rewrite Heqt, Heqres in Hequiv.
+        inversion Hequiv as [t' ms'' gl'' dir' res' Hequiv' Heqt' Heqms'' Heqgl'' Heqdir' Heqres' | |].
+        clear t' ms'' gl'' res' Heqt' Heqms'' Heqgl'' Heqres'.
+        rewrite Heqms' in Hequiv'. rewrite Hy_ms_sameinp. rewrite Hmsstr0 in Hequiv'.
+        assumption.
+      }
+      specialize (IH ms Hmsstr0). simpl in *.
+      destruct (tmsub ms treecont) as [t|] eqn:Heqt; simpl. 2: constructor.
+      destruct (msub ms origcont) as [res|] eqn:Heqres; simpl. 2: constructor.
+      constructor. inversion IH. auto.
+
+    - (* Input start *)
+      simpl. intros _ m tm dir Heqm Heqtm. injection Heqm as <-. injection Heqtm as <-.
+      intro str0. unfold equiv_tree_matcher. intros mc tmc gl Hequivcont.
+      unfold equiv_tree_mcont. intros ms Hmsstr0.
+      destruct (if (_: bool) then Success true else _) as [anchormatch|]; simpl. 2: constructor.
+      destruct anchormatch.
+      + unfold equiv_tree_mcont in Hequivcont. specialize (Hequivcont ms Hmsstr0). inversion Hequivcont; try solve[constructor]; simpl.
+        constructor. auto.
+      + constructor. auto.
+
+    - (* Input end: same as input start, but the placeholders in the first destruct are different *)
+      simpl. intros _ m tm dir Heqm Heqtm. injection Heqm as <-. injection Heqtm as <-.
+      intros str0 mc tmc gl Hequivcont ms Hmsstr0.
+      destruct (if (_: bool) then Success true else _) as [anchormatch|]; simpl. 2: constructor.
+      destruct anchormatch.
+      + unfold equiv_tree_mcont in Hequivcont. specialize (Hequivcont ms Hmsstr0). inversion Hequivcont; try solve[constructor]; simpl.
+        constructor. auto.
+      + constructor. auto.
+
+    (* Word boundary *)
+    - simpl. intros _ m tm dir Hcompsucc Htcompsucc str0. injection Hcompsucc as <-. injection Htcompsucc as <-.
+      unfold equiv_tree_matcher.
+      intros mc tmc gl Hequivcont. unfold equiv_tree_mcont.
+      intros ms Hmsstr0.
+      destruct Semantics.isWordChar as [a|] eqn:Hwca; simpl. 2: constructor.
+      destruct (Semantics.isWordChar rer (_ ms) (MatchState.endIndex ms)) as [b|] eqn:Hwcb; simpl. 2: constructor.
+      destruct (_ && _ || _ && _); simpl.
+      + unfold equiv_tree_mcont in Hequivcont. specialize (Hequivcont ms Hmsstr0).
+        destruct tmc as [t|]; simpl. 2: constructor.
+        destruct mc as [res|]; simpl. 2: constructor.
+        constructor. simpl. now inversion Hequivcont.
+      + constructor. reflexivity.
+
+    (* Non word boundary; same proof as above, except the placeholders at the main destruct differ *)
+    - simpl. intros _ m tm dir Hcompsucc Htcompsucc str0. injection Hcompsucc as <-. injection Htcompsucc as <-.
+      unfold equiv_tree_matcher.
+      intros mc tmc gl Hequivcont. unfold equiv_tree_mcont.
+      intros ms Hmsstr0.
+      destruct Semantics.isWordChar as [a|] eqn:Hwca; simpl. 2: constructor.
+      destruct (Semantics.isWordChar rer (_ ms) (MatchState.endIndex ms)) as [b|] eqn:Hwcb; simpl. 2: constructor.
+      destruct (_ && _ || _ && _); simpl.
+      + unfold equiv_tree_mcont in Hequivcont. specialize (Hequivcont ms Hmsstr0).
+        destruct tmc as [t|]; simpl. 2: constructor.
+        destruct mc as [res|]; simpl. 2: constructor.
+        constructor. simpl. now inversion Hequivcont.
+      + constructor. reflexivity.
+
+      (* Positive lookahead *)
+    - simpl. intros. apply compile_tcompile_lk with (lkdir := forward) (pos := true) (lkreg := wr) (rer := rer) (ctx := ctx); auto.
+
+      (* Negative lookahead *)
+    - simpl. intros. apply compile_tcompile_lk with (lkdir := forward) (pos := false) (lkreg := wr) (rer := rer) (ctx := ctx); auto.
+
+      (* Positive lookbehind *)
+    - simpl. intros. apply compile_tcompile_lk with (lkdir := backward) (pos := true) (lkreg := wr) (rer := rer) (ctx := ctx); auto.
+
+      (* Negative lookbehind *)
+    - simpl. intros. apply compile_tcompile_lk with (lkdir := backward) (pos := false) (lkreg := wr) (rer := rer) (ctx := ctx); auto.
+  Qed.
+End LWEquivTMatcher.
