warblreequiv/LindenParameters.v
@@ -8,171 +8,162 @@ Import Utils.List.
 Local Open Scope bool_scope.
 
 
-(** * Instantiation of Warblre typeclasses Character, String, Property (Unicode) with Linden types *)
+(** * Instantiation of Warblre typeclasses String, Property (Unicode) *)
 
-(** ** Characters *)
+Section LindenParameters.
+  Context `{characterClass: Character.class}.
+  
 
-(* We axiomatize most required parameters *)
-Instance char_eqdec: EqDec Char := {| EqDec.eq_dec := char_eq_dec |}.
-Parameter char_canonicalize: RegExpRecord -> Char -> Char.
-
-(* As per the ECMA specification (22.2.2.7.3 Canonicalize ( rer, ch )), when we do not ignore case, canonicalization is the identity function. *)
-Axiom canonicalize_casesenst: forall rer chr, RegExpRecord.ignoreCase rer = false -> char_canonicalize rer chr = chr.
-
-Instance CharCharacter: Character.class :=
-  Character.make Char char_eqdec char_from_numeric_value char_numeric_value
-  char_canonicalize char_all char_line_terminators char_digits
-  char_white_spaces char_ascii_word_characters char_numeric_pseudo_bij
-  char_numeric_round_trip_order.
+  (* As per the ECMA specification (22.2.2.7.3 Canonicalize ( rer, ch )), when we do not ignore case, canonicalization is the identity function. *)
+  Axiom canonicalize_casesenst: forall rer chr, RegExpRecord.ignoreCase rer = false -> Character.canonicalize rer chr = chr.
 
 
+  (** ** Strings *)
 
-(** ** Strings *)
+  (* Adapted from String.substring: returns the substring of s starting at index n and of length m (or less if the string is not long enough). *)
+  Fixpoint substring (s: string) (n m: nat): string :=
+    match n, m, s with
+    | 0, 0, _ => nil
+    | 0, S m', nil => s
+    | 0, S m', c::s' => c::substring s' 0 m'
+    | S n', _, nil => s
+    | S n', _, c::s' => substring s' n' m
+    end.
 
-Instance string_eqdec: EqDec string := {| EqDec.eq_dec := string_eq_dec |}.
+  Definition advanceStringIndex (s: string) (i: nat) := S i.
+  Definition getStringIndex (s: string) (i: nat) := i.
+  (* Linden strings are just lists of characters *)
+  Definition to_char_list (s: string): list Character := s.
 
-(* Adapted from String.substring: returns the substring of s starting at index n and of length m (or less if the string is not long enough). *)
-Fixpoint substring (s: string) (n m: nat): string :=
-  match n, m, s with
-  | 0, 0, _ => nil
-  | 0, S m', nil => s
-  | 0, S m', c::s' => c::substring s' 0 m'
-  | S n', _, nil => s
-  | S n', _, c::s' => substring s' n' m
-  end.
-
-Definition advanceStringIndex (s: string) (i: nat) := S i.
-Definition getStringIndex (s: string) (i: nat) := i.
-(* Linden strings are just lists of characters *)
-Definition to_char_list (s: string): list Char := s.
-
-Instance string_String: String.class Char := {|
-  String.type := string;
-  String.eqdec := string_eqdec;
-  String.length := @List.length Char;
-  String.substring := substring;
-  String.advanceStringIndex := advanceStringIndex;
-  String.getStringIndex := getStringIndex;
-  String.to_char_list := to_char_list
-|}.
-
-
-
-(** ** Unicode properties *)
-(* We don't support Unicode properties *)
-Inductive NoProperty: Type := .
-
-Definition NoProp_code_points_for (p: NoProperty): list Char := match p with end.
-
-#[refine] Instance NoPropertyProp: Property.class Char := {|
-  Property.type := NoProperty;
-  Property.code_points_for := NoProp_code_points_for
-|}.
-Proof.
-  constructor. decide equality.
-Defined.
-
-
-
-(** ** Type markers *)
-Instance char_marker: CharacterMarker Char := mk_character_marker Char.
-
-Instance string_marker: StringMarker string := mk_string_marker string.
-
-Instance empty_unicode_marker: UnicodePropertyMarker NoProperty := mk_unicode_property_marker NoProperty.
-
-
-(** ** Parameters typeclass *)
-Parameter linden_set_class: @CharSet.class CharCharacter.
-
-Instance LindenParameters: Parameters := {|
-    Parameters.character_class := CharCharacter;
-
-    Parameters.set_class := linden_set_class;
-    Parameters.string_class := string_String;
-    Parameters.unicode_property_class := NoPropertyProp;
-
-    Parameters.character_marker := char_marker;
-    Parameters.string_marker := string_marker;
-    Parameters.unicode_property_marker := empty_unicode_marker
+  #[export] Instance string_String: String.class Character := {|
+    String.type := string;
+    String.eqdec := string_EqDec;
+    String.length := @List.length Character;
+    String.substring := substring;
+    String.advanceStringIndex := advanceStringIndex;
+    String.getStringIndex := getStringIndex;
+    String.to_char_list := to_char_list
   |}.
 
 
-(** ** Axiomatization of CharSet *)
-Axiom charset_empty_contains: forall c: Char, CharSet.contains CharSet.empty c = false.
-Axiom charset_from_list_contains: forall (c: Char) (l: list Char), CharSet.contains (CharSet.from_list l) c = true <-> In c l.
-Axiom charset_union_contains: forall (c: Char) (s t: CharSet), CharSet.contains (CharSet.union s t) c = CharSet.contains s c || CharSet.contains t c.
-(* Singleton? *)
-(* Size? *)
-Axiom charset_remove_all_contains: forall (c: Char) (s t: CharSet), CharSet.contains (CharSet.remove_all s t) c = CharSet.contains s c && negb (CharSet.contains t c).
-Axiom charset_is_empty_iff: forall s: CharSet, CharSet.is_empty s = true <-> s = CharSet.empty.
-(* Range? *)
-Axiom charset_unique_iff:
-  forall {F: Type} {af: Result.AssertionError F} (s: CharSet) (c: Char),
-    @CharSet.unique _ _ F af s = Success c <-> forall c': Char, CharSet.contains s c' = true <-> c' = c.
-Axiom charset_filter_contains:
-  forall (s: CharSet) (f: Char -> bool) (c: Char),
-    CharSet.contains (CharSet.filter s f) c = CharSet.contains s c && f c.
-Axiom charset_exist_iff:
-  forall (s: CharSet) (f: Char -> bool),
-    CharSet.exist s f = true <-> exists c: Char, CharSet.contains s c = true /\ f c = true.
 
-(* Do we need extensionality? *)
-Axiom charset_ext:
-  forall s t: CharSet,
-    s = t <-> forall c: Char, CharSet.contains s c = CharSet.contains t c.
+  (** ** Unicode properties *)
+  (* We don't support Unicode properties *)
+  Inductive NoProperty: Type := .
+
+  Definition NoProp_code_points_for (p: NoProperty): list Character := match p with end.
+
+  #[refine,export] Instance NoPropertyProp: Property.class Character := {|
+    Property.type := NoProperty;
+    Property.code_points_for := NoProp_code_points_for
+  |}.
+  Proof.
+    constructor. decide equality.
+  Defined.
 
 
-(* Lemmas following from above axioms *)
-Lemma charset_exist_false_iff:
-  forall (s: CharSet) (f: Char -> bool),
-    CharSet.exist s f = false <-> forall c: Char, CharSet.contains s c = false \/ f c = false.
-Proof.
-  intros s f. split.
-  - intros H c. destruct CharSet.contains eqn:Hcontains; destruct f eqn:Hfilter; auto.
-    assert (exists c, CharSet.contains s c = true /\ f c = true) as Hexist. { exists c. auto. }
-    rewrite <- charset_exist_iff in Hexist. congruence.
-  - intro H. destruct CharSet.exist eqn:Hexist; auto.
-    rewrite charset_exist_iff in Hexist. destruct Hexist as [c [Hcontains Hfilter]].
-    specialize (H c). destruct H; congruence.
-Qed.
 
-Lemma charset_from_list_contains_inb: forall (c: Char) (l: list Char), CharSet.contains (CharSet.from_list l) c = inb c l.
-Proof.
-  intros c l.
-  apply <- Bool.eq_iff_eq_true. rewrite inb_spec. apply charset_from_list_contains.
-Qed.
+  (** ** Type markers *)
+  #[export] Instance char_marker: CharacterMarker Character := mk_character_marker Character.
 
-Lemma charset_union_empty:
-  forall s, CharSet.union s CharSet.empty = s.
-Proof.
-  intro s. apply <- charset_ext. intro c.
-  rewrite charset_union_contains, charset_empty_contains. apply Bool.orb_false_r.
-Qed.
+  #[export] Instance string_marker: StringMarker string := mk_string_marker string.
 
-Lemma charset_contains_singleton_self:
-  forall c, CharSet.contains (CharSet.singleton c) c = true.
-Proof.
-  intro c.
-  set (p := fun chr => (chr ==? c)%wt).
-  assert (Hexist: CharSet.exist (CharSet.singleton c) p = true). {
-    rewrite CharSet.singleton_exist. unfold p. apply EqDec.reflb.
-  }
-  rewrite charset_exist_iff in Hexist. destruct Hexist as [chr [Hcontains Heq]].
-  unfold p in Heq. rewrite EqDec.inversion_true in Heq. subst chr. assumption.
-Qed.
-  
+  #[export] Instance empty_unicode_marker: UnicodePropertyMarker NoProperty := mk_unicode_property_marker NoProperty.
 
-Lemma charset_contains_singleton:
-  forall c chr, CharSet.contains (CharSet.singleton c) chr = (chr ==? c)%wt.
-Proof.
-  intros c chr.
-  apply Bool.eq_true_iff_eq. split.
-  - intro Hcontains. set (f := fun c' => (chr ==? c')%wt).
-    assert (H: exists chr0, CharSet.contains (CharSet.singleton c) chr0 = true /\ f chr0 = true). {
-      exists chr. split; auto. unfold f. apply EqDec.reflb.
+
+  (** ** Parameters typeclass *)
+  Parameter linden_set_class: @CharSet.class characterClass.
+
+  #[export] Instance LindenParameters: Parameters := {|
+      Parameters.character_class := characterClass;
+
+      Parameters.set_class := linden_set_class;
+      Parameters.string_class := string_String;
+      Parameters.unicode_property_class := NoPropertyProp;
+
+      Parameters.character_marker := char_marker;
+      Parameters.string_marker := string_marker;
+      Parameters.unicode_property_marker := empty_unicode_marker
+    |}.
+
+
+  (** ** Axiomatization of CharSet *)
+  Axiom charset_empty_contains: forall c: Character, CharSet.contains CharSet.empty c = false.
+  Axiom charset_from_list_contains: forall (c: Character) (l: list Character), CharSet.contains (CharSet.from_list l) c = true <-> In c l.
+  Axiom charset_union_contains: forall (c: Character) (s t: CharSet), CharSet.contains (CharSet.union s t) c = CharSet.contains s c || CharSet.contains t c.
+  (* Singleton? *)
+  (* Size? *)
+  Axiom charset_remove_all_contains: forall (c: Character) (s t: CharSet), CharSet.contains (CharSet.remove_all s t) c = CharSet.contains s c && negb (CharSet.contains t c).
+  Axiom charset_is_empty_iff: forall s: CharSet, CharSet.is_empty s = true <-> s = CharSet.empty.
+  (* Range? *)
+  Axiom charset_unique_iff:
+    forall {F: Type} {af: Result.AssertionError F} (s: CharSet) (c: Character),
+      @CharSet.unique _ _ F af s = Success c <-> forall c': Character, CharSet.contains s c' = true <-> c' = c.
+  Axiom charset_filter_contains:
+    forall (s: CharSet) (f: Character -> bool) (c: Character),
+      CharSet.contains (CharSet.filter s f) c = CharSet.contains s c && f c.
+  Axiom charset_exist_iff:
+    forall (s: CharSet) (f: Character -> bool),
+      CharSet.exist s f = true <-> exists c: Character, CharSet.contains s c = true /\ f c = true.
+
+  (* Do we need extensionality? *)
+  Axiom charset_ext:
+    forall s t: CharSet,
+      s = t <-> forall c: Character, CharSet.contains s c = CharSet.contains t c.
+
+
+  (* Lemmas following from above axioms *)
+  Lemma charset_exist_false_iff:
+    forall (s: CharSet) (f: Character -> bool),
+      CharSet.exist s f = false <-> forall c: Character, CharSet.contains s c = false \/ f c = false.
+  Proof.
+    intros s f. split.
+    - intros H c. destruct CharSet.contains eqn:Hcontains; destruct f eqn:Hfilter; auto.
+      assert (exists c, CharSet.contains s c = true /\ f c = true) as Hexist. { exists c. auto. }
+      rewrite <- charset_exist_iff in Hexist. congruence.
+    - intro H. destruct CharSet.exist eqn:Hexist; auto.
+      rewrite charset_exist_iff in Hexist. destruct Hexist as [c [Hcontains Hfilter]].
+      specialize (H c). destruct H; congruence.
+  Qed.
+
+  Lemma charset_from_list_contains_inb: forall (c: Character) (l: list Character), CharSet.contains (CharSet.from_list l) c = inb c l.
+  Proof.
+    intros c l.
+    apply <- Bool.eq_iff_eq_true. rewrite inb_spec. apply charset_from_list_contains.
+  Qed.
+
+  Lemma charset_union_empty:
+    forall s, CharSet.union s CharSet.empty = s.
+  Proof.
+    intro s. apply <- charset_ext. intro c.
+    rewrite charset_union_contains, charset_empty_contains. apply Bool.orb_false_r.
+  Qed.
+
+  Lemma charset_contains_singleton_self:
+    forall c, CharSet.contains (CharSet.singleton c) c = true.
+  Proof.
+    intro c.
+    set (p := fun chr => (chr ==? c)%wt).
+    assert (Hexist: CharSet.exist (CharSet.singleton c) p = true). {
+      rewrite CharSet.singleton_exist. unfold p. apply EqDec.reflb.
     }
-    rewrite <- charset_exist_iff in H. rewrite CharSet.singleton_exist in H.
-    apply H.
-  - intro Heq. rewrite EqDec.inversion_true in Heq. subst chr. apply charset_contains_singleton_self.
-Qed.
+    rewrite charset_exist_iff in Hexist. destruct Hexist as [chr [Hcontains Heq]].
+    unfold p in Heq. rewrite EqDec.inversion_true in Heq. subst chr. assumption.
+  Qed.
+
+
+  Lemma charset_contains_singleton:
+    forall c chr, CharSet.contains (CharSet.singleton c) chr = (chr ==? c)%wt.
+  Proof.
+    intros c chr.
+    apply Bool.eq_true_iff_eq. split.
+    - intro Hcontains. set (f := fun c' => (chr ==? c')%wt).
+      assert (H: exists chr0, CharSet.contains (CharSet.singleton c) chr0 = true /\ f chr0 = true). {
+        exists chr. split; auto. unfold f. apply EqDec.reflb.
+      }
+      rewrite <- charset_exist_iff in H. rewrite CharSet.singleton_exist in H.
+      apply H.
+    - intro Heq. rewrite EqDec.inversion_true in Heq. subst chr. apply charset_contains_singleton_self.
+  Qed.
+
+End LindenParameters.
